Wip Binencoder with dns example

src/BinEncoders/Examples/Extracted.ml
@@ -1,0 +1,3143 @@
+type __ = Obj.t
+let __ = let rec f _ = Obj.repr f in Obj.repr f
+
+(** val negb : bool -> bool **)
+
+let negb = function
+| true -> false
+| false -> true
+
+type nat =
+| O
+| S of nat
+
+(** val fst : ('a1*'a2) -> 'a1 **)
+
+let fst = function
+| x,y -> x
+
+(** val snd : ('a1*'a2) -> 'a2 **)
+
+let snd = function
+| x,y -> y
+
+(** val length : 'a1 list -> nat **)
+
+let rec length = function
+| [] -> O
+| y::l' -> S (length l')
+
+(** val app : 'a1 list -> 'a1 list -> 'a1 list **)
+
+let rec app l m =
+  match l with
+  | [] -> m
+  | a::l1 -> a::(app l1 m)
+
+type comparison =
+| Eq
+| Lt
+| Gt
+
+type compareSpecT =
+| CompEqT
+| CompLtT
+| CompGtT
+
+(** val compareSpec2Type : comparison -> compareSpecT **)
+
+let compareSpec2Type = function
+| Eq -> CompEqT
+| Lt -> CompLtT
+| Gt -> CompGtT
+
+type 'a compSpecT = compareSpecT
+
+(** val compSpec2Type : 'a1 -> 'a1 -> comparison -> 'a1 compSpecT **)
+
+let compSpec2Type x y c =
+  compareSpec2Type c
+
+type 'a sig0 =
+  'a
+  (* singleton inductive, whose constructor was exist *)
+
+type 'a sumor =
+| Inleft of 'a
+| Inright
+
+(** val pred : nat -> nat **)
+
+let pred n0 = match n0 with
+| O -> n0
+| S u -> u
+
+(** val plus : nat -> nat -> nat **)
+
+let rec plus n0 m =
+  match n0 with
+  | O -> m
+  | S p -> S (plus p m)
+
+(** val minus : nat -> nat -> nat **)
+
+let rec minus n0 m =
+  match n0 with
+  | O -> n0
+  | S k ->
+    (match m with
+     | O -> n0
+     | S l -> minus k l)
+
+(** val min : nat -> nat -> nat **)
+
+let rec min n0 m =
+  match n0 with
+  | O -> O
+  | S n' ->
+    (match m with
+     | O -> O
+     | S m' -> S (min n' m'))
+
+(** val nat_iter : nat -> ('a1 -> 'a1) -> 'a1 -> 'a1 **)
+
+let rec nat_iter n0 f x =
+  match n0 with
+  | O -> x
+  | S n' -> f (nat_iter n' f x)
+
+type reflect =
+| ReflectT
+| ReflectF
+
+(** val iff_reflect : bool -> reflect **)
+
+let iff_reflect = function
+| true -> ReflectT
+| false -> ReflectF
+
+type ('data_t, 'bin_t) decoder =
+  'bin_t -> 'data_t
+  (* singleton inductive, whose constructor was Build_decoder *)
+
+(** val decode : ('a1 -> 'a2) -> ('a1, 'a2) decoder -> 'a2 -> 'a1 **)
+
+let decode encode decoder0 =
+  decoder0
+
+(** val decode_unpack :
+    ('a1 -> 'a3) -> (('a3*'a2) -> 'a2) -> ('a1 -> 'a2) -> ('a3*'a2, 'a2)
+    decoder -> ('a3 -> ('a1, 'a2) decoder) -> ('a1, 'a2) decoder **)
+
+let decode_unpack project encode1 encode2 decoder1 decoder2 bin =
+  let proj,ext = decode encode1 decoder1 bin in
+  decode encode2 (decoder2 proj) ext
+
+(** val strengthen_Decoder :
+    ('a1 -> 'a2) -> ('a1, 'a2) decoder -> ('a1, 'a2) decoder **)
+
+let strengthen_Decoder encode_data data_decoder =
+  decode encode_data data_decoder
+
+(** val nested_decoder :
+    ('a1 -> 'a2) -> ('a2 -> 'a3) -> ('a1, 'a2) decoder -> ('a2, 'a3)
+    decoder -> ('a1, 'a3) decoder **)
+
+let nested_decoder encodeA encodeB a_decoder b_decoder c =
+  decode encodeA a_decoder (decode encodeB b_decoder c)
+
+(** val unprod_decoder :
+    ('a1 -> 'a2) -> ('a1, 'a2) decoder -> ('a1*'a3, 'a2*'a3) decoder **)
+
+let unprod_decoder encodeA a_decoder bundle =
+  (decode encodeA a_decoder (fst bundle)),(snd bundle)
+
+type bin_t = bool list
+
+(** val bin_encode_transform_pair :
+    ('a1 -> bin_t) -> ('a1*bin_t) -> bool list **)
+
+let bin_encode_transform_pair encode = function
+| _data,_bin -> app (encode _data) _bin
+
+(** val bin_encode_transform_pair_Decoder :
+    ('a1 -> bin_t) -> (bin_t -> 'a1*bin_t) -> ('a1*bin_t, bool list)
+    decoder **)
+
+let bin_encode_transform_pair_Decoder encode decode0 =
+  decode0
+
+type positive =
+| XI of positive
+| XO of positive
+| XH
+
+type n =
+| N0
+| Npos of positive
+
+module Pos =
+ struct
+  type t = positive
+
+  (** val succ : positive -> positive **)
+
+  let rec succ = function
+  | XI p -> XO (succ p)
+  | XO p -> XI p
+  | XH -> XO XH
+
+  (** val add : positive -> positive -> positive **)
+
+  let rec add x y =
+    match x with
+    | XI p ->
+      (match y with
+       | XI q -> XO (add_carry p q)
+       | XO q -> XI (add p q)
+       | XH -> XO (succ p))
+    | XO p ->
+      (match y with
+       | XI q -> XI (add p q)
+       | XO q -> XO (add p q)
+       | XH -> XI p)
+    | XH ->
+      (match y with
+       | XI q -> XO (succ q)
+       | XO q -> XI q
+       | XH -> XO XH)
+
+  (** val add_carry : positive -> positive -> positive **)
+
+  and add_carry x y =
+    match x with
+    | XI p ->
+      (match y with
+       | XI q -> XI (add_carry p q)
+       | XO q -> XO (add_carry p q)
+       | XH -> XI (succ p))
+    | XO p ->
+      (match y with
+       | XI q -> XO (add_carry p q)
+       | XO q -> XI (add p q)
+       | XH -> XO (succ p))
+    | XH ->
+      (match y with
+       | XI q -> XI (succ q)
+       | XO q -> XO (succ q)
+       | XH -> XI XH)
+
+  (** val pred_double : positive -> positive **)
+
+  let rec pred_double = function
+  | XI p -> XI (XO p)
+  | XO p -> XI (pred_double p)
+  | XH -> XH
+
+  (** val pred : positive -> positive **)
+
+  let pred = function
+  | XI p -> XO p
+  | XO p -> pred_double p
+  | XH -> XH
+
+  (** val pred_N : positive -> n **)
+
+  let pred_N = function
+  | XI p -> Npos (XO p)
+  | XO p -> Npos (pred_double p)
+  | XH -> N0
+
+  type mask =
+  | IsNul
+  | IsPos of positive
+  | IsNeg
+
+  (** val mask_rect : 'a1 -> (positive -> 'a1) -> 'a1 -> mask -> 'a1 **)
+
+  let mask_rect f f0 f1 = function
+  | IsNul -> f
+  | IsPos x -> f0 x
+  | IsNeg -> f1
+
+  (** val mask_rec : 'a1 -> (positive -> 'a1) -> 'a1 -> mask -> 'a1 **)
+
+  let mask_rec f f0 f1 = function
+  | IsNul -> f
+  | IsPos x -> f0 x
+  | IsNeg -> f1
+
+  (** val succ_double_mask : mask -> mask **)
+
+  let succ_double_mask = function
+  | IsNul -> IsPos XH
+  | IsPos p -> IsPos (XI p)
+  | IsNeg -> IsNeg
+
+  (** val double_mask : mask -> mask **)
+
+  let double_mask = function
+  | IsPos p -> IsPos (XO p)
+  | x0 -> x0
+
+  (** val double_pred_mask : positive -> mask **)
+
+  let double_pred_mask = function
+  | XI p -> IsPos (XO (XO p))
+  | XO p -> IsPos (XO (pred_double p))
+  | XH -> IsNul
+
+  (** val pred_mask : mask -> mask **)
+
+  let pred_mask = function
+  | IsPos q ->
+    (match q with
+     | XH -> IsNul
+     | _ -> IsPos (pred q))
+  | _ -> IsNeg
+
+  (** val sub_mask : positive -> positive -> mask **)
+
+  let rec sub_mask x y =
+    match x with
+    | XI p ->
+      (match y with
+       | XI q -> double_mask (sub_mask p q)
+       | XO q -> succ_double_mask (sub_mask p q)
+       | XH -> IsPos (XO p))
+    | XO p ->
+      (match y with
+       | XI q -> succ_double_mask (sub_mask_carry p q)
+       | XO q -> double_mask (sub_mask p q)
+       | XH -> IsPos (pred_double p))
+    | XH ->
+      (match y with
+       | XH -> IsNul
+       | _ -> IsNeg)
+
+  (** val sub_mask_carry : positive -> positive -> mask **)
+
+  and sub_mask_carry x y =
+    match x with
+    | XI p ->
+      (match y with
+       | XI q -> succ_double_mask (sub_mask_carry p q)
+       | XO q -> double_mask (sub_mask p q)
+       | XH -> IsPos (pred_double p))
+    | XO p ->
+      (match y with
+       | XI q -> double_mask (sub_mask_carry p q)
+       | XO q -> succ_double_mask (sub_mask_carry p q)
+       | XH -> double_pred_mask p)
+    | XH -> IsNeg
+
+  (** val sub : positive -> positive -> positive **)
+
+  let sub x y =
+    match sub_mask x y with
+    | IsPos z -> z
+    | _ -> XH
+
+  (** val mul : positive -> positive -> positive **)
+
+  let rec mul x y =
+    match x with
+    | XI p -> add y (XO (mul p y))
+    | XO p -> XO (mul p y)
+    | XH -> y
+
+  (** val iter : positive -> ('a1 -> 'a1) -> 'a1 -> 'a1 **)
+
+  let rec iter n0 f x =
+    match n0 with
+    | XI n' -> f (iter n' f (iter n' f x))
+    | XO n' -> iter n' f (iter n' f x)
+    | XH -> f x
+
+  (** val pow : positive -> positive -> positive **)
+
+  let pow x y =
+    iter y (mul x) XH
+
+  (** val square : positive -> positive **)
+
+  let rec square = function
+  | XI p0 -> XI (XO (add (square p0) p0))
+  | XO p0 -> XO (XO (square p0))
+  | XH -> XH
+
+  (** val div2 : positive -> positive **)
+
+  let div2 = function
+  | XI p0 -> p0
+  | XO p0 -> p0
+  | XH -> XH
+
+  (** val div2_up : positive -> positive **)
+
+  let div2_up = function
+  | XI p0 -> succ p0
+  | XO p0 -> p0
+  | XH -> XH
+
+  (** val size_nat : positive -> nat **)
+
+  let rec size_nat = function
+  | XI p0 -> S (size_nat p0)
+  | XO p0 -> S (size_nat p0)
+  | XH -> S O
+
+  (** val size : positive -> positive **)
+
+  let rec size = function
+  | XI p0 -> succ (size p0)
+  | XO p0 -> succ (size p0)
+  | XH -> XH
+
+  (** val compare_cont :
+      positive -> positive -> comparison -> comparison **)
+
+  let rec compare_cont x y r =
+    match x with
+    | XI p ->
+      (match y with
+       | XI q -> compare_cont p q r
+       | XO q -> compare_cont p q Gt
+       | XH -> Gt)
+    | XO p ->
+      (match y with
+       | XI q -> compare_cont p q Lt
+       | XO q -> compare_cont p q r
+       | XH -> Gt)
+    | XH ->
+      (match y with
+       | XH -> r
+       | _ -> Lt)
+
+  (** val compare : positive -> positive -> comparison **)
+
+  let compare x y =
+    compare_cont x y Eq
+
+  (** val min : positive -> positive -> positive **)
+
+  let min p p' =
+    match compare p p' with
+    | Gt -> p'
+    | _ -> p
+
+  (** val max : positive -> positive -> positive **)
+
+  let max p p' =
+    match compare p p' with
+    | Gt -> p
+    | _ -> p'
+
+  (** val eqb : positive -> positive -> bool **)
+
+  let rec eqb p q =
+    match p with
+    | XI p0 ->
+      (match q with
+       | XI q0 -> eqb p0 q0
+       | _ -> false)
+    | XO p0 ->
+      (match q with
+       | XO q0 -> eqb p0 q0
+       | _ -> false)
+    | XH ->
+      (match q with
+       | XH -> true
+       | _ -> false)
+
+  (** val leb : positive -> positive -> bool **)
+
+  let leb x y =
+    match compare x y with
+    | Gt -> false
+    | _ -> true
+
+  (** val ltb : positive -> positive -> bool **)
+
+  let ltb x y =
+    match compare x y with
+    | Lt -> true
+    | _ -> false
+
+  (** val sqrtrem_step :
+      (positive -> positive) -> (positive -> positive) -> (positive*mask)
+      -> positive*mask **)
+
+  let sqrtrem_step f g = function
+  | s,y ->
+    (match y with
+     | IsPos r ->
+       let s' = XI (XO s) in
+       let r' = g (f r) in
+       if leb s' r' then (XI s),(sub_mask r' s') else (XO s),(IsPos r')
+     | _ -> (XO s),(sub_mask (g (f XH)) (XO (XO XH))))
+
+  (** val sqrtrem : positive -> positive*mask **)
+
+  let rec sqrtrem = function
+  | XI p0 ->
+    (match p0 with
+     | XI p1 -> sqrtrem_step (fun x -> XI x) (fun x -> XI x) (sqrtrem p1)
+     | XO p1 -> sqrtrem_step (fun x -> XO x) (fun x -> XI x) (sqrtrem p1)
+     | XH -> XH,(IsPos (XO XH)))
+  | XO p0 ->
+    (match p0 with
+     | XI p1 -> sqrtrem_step (fun x -> XI x) (fun x -> XO x) (sqrtrem p1)
+     | XO p1 -> sqrtrem_step (fun x -> XO x) (fun x -> XO x) (sqrtrem p1)
+     | XH -> XH,(IsPos XH))
+  | XH -> XH,IsNul
+
+  (** val sqrt : positive -> positive **)
+
+  let sqrt p =
+    fst (sqrtrem p)
+
+  (** val gcdn : nat -> positive -> positive -> positive **)
+
+  let rec gcdn n0 a b =
+    match n0 with
+    | O -> XH
+    | S n1 ->
+      (match a with
+       | XI a' ->
+         (match b with
+          | XI b' ->
+            (match compare a' b' with
+             | Eq -> a
+             | Lt -> gcdn n1 (sub b' a') a
+             | Gt -> gcdn n1 (sub a' b') b)
+          | XO b0 -> gcdn n1 a b0
+          | XH -> XH)
+       | XO a0 ->
+         (match b with
+          | XI p -> gcdn n1 a0 b
+          | XO b0 -> XO (gcdn n1 a0 b0)
+          | XH -> XH)
+       | XH -> XH)
+
+  (** val gcd : positive -> positive -> positive **)
+
+  let gcd a b =
+    gcdn (plus (size_nat a) (size_nat b)) a b
+
+  (** val ggcdn :
+      nat -> positive -> positive -> positive*(positive*positive) **)
+
+  let rec ggcdn n0 a b =
+    match n0 with
+    | O -> XH,(a,b)
+    | S n1 ->
+      (match a with
+       | XI a' ->
+         (match b with
+          | XI b' ->
+            (match compare a' b' with
+             | Eq -> a,(XH,XH)
+             | Lt ->
+               let g,p = ggcdn n1 (sub b' a') a in
+               let ba,aa = p in g,(aa,(add aa (XO ba)))
+             | Gt ->
+               let g,p = ggcdn n1 (sub a' b') b in
+               let ab,bb = p in g,((add bb (XO ab)),bb))
+          | XO b0 ->
+            let g,p = ggcdn n1 a b0 in let aa,bb = p in g,(aa,(XO bb))
+          | XH -> XH,(a,XH))
+       | XO a0 ->
+         (match b with
+          | XI p ->
+            let g,p0 = ggcdn n1 a0 b in let aa,bb = p0 in g,((XO aa),bb)
+          | XO b0 -> let g,p = ggcdn n1 a0 b0 in (XO g),p
+          | XH -> XH,(a,XH))
+       | XH -> XH,(XH,b))
+
+  (** val ggcd : positive -> positive -> positive*(positive*positive) **)
+
+  let ggcd a b =
+    ggcdn (plus (size_nat a) (size_nat b)) a b
+
+  (** val coq_Nsucc_double : n -> n **)
+
+  let coq_Nsucc_double = function
+  | N0 -> Npos XH
+  | Npos p -> Npos (XI p)
+
+  (** val coq_Ndouble : n -> n **)
+
+  let coq_Ndouble = function
+  | N0 -> N0
+  | Npos p -> Npos (XO p)
+
+  (** val coq_lor : positive -> positive -> positive **)
+
+  let rec coq_lor p q =
+    match p with
+    | XI p0 ->
+      (match q with
+       | XI q0 -> XI (coq_lor p0 q0)
+       | XO q0 -> XI (coq_lor p0 q0)
+       | XH -> p)
+    | XO p0 ->
+      (match q with
+       | XI q0 -> XI (coq_lor p0 q0)
+       | XO q0 -> XO (coq_lor p0 q0)
+       | XH -> XI p0)
+    | XH ->
+      (match q with
+       | XO q0 -> XI q0
+       | _ -> q)
+
+  (** val coq_land : positive -> positive -> n **)
+
+  let rec coq_land p q =
+    match p with
+    | XI p0 ->
+      (match q with
+       | XI q0 -> coq_Nsucc_double (coq_land p0 q0)
+       | XO q0 -> coq_Ndouble (coq_land p0 q0)
+       | XH -> Npos XH)
+    | XO p0 ->
+      (match q with
+       | XI q0 -> coq_Ndouble (coq_land p0 q0)
+       | XO q0 -> coq_Ndouble (coq_land p0 q0)
+       | XH -> N0)
+    | XH ->
+      (match q with
+       | XO q0 -> N0
+       | _ -> Npos XH)
+
+  (** val ldiff : positive -> positive -> n **)
+
+  let rec ldiff p q =
+    match p with
+    | XI p0 ->
+      (match q with
+       | XI q0 -> coq_Ndouble (ldiff p0 q0)
+       | XO q0 -> coq_Nsucc_double (ldiff p0 q0)
+       | XH -> Npos (XO p0))
+    | XO p0 ->
+      (match q with
+       | XI q0 -> coq_Ndouble (ldiff p0 q0)
+       | XO q0 -> coq_Ndouble (ldiff p0 q0)
+       | XH -> Npos p)
+    | XH ->
+      (match q with
+       | XO q0 -> Npos XH
+       | _ -> N0)
+
+  (** val coq_lxor : positive -> positive -> n **)
+
+  let rec coq_lxor p q =
+    match p with
+    | XI p0 ->
+      (match q with
+       | XI q0 -> coq_Ndouble (coq_lxor p0 q0)
+       | XO q0 -> coq_Nsucc_double (coq_lxor p0 q0)
+       | XH -> Npos (XO p0))
+    | XO p0 ->
+      (match q with
+       | XI q0 -> coq_Nsucc_double (coq_lxor p0 q0)
+       | XO q0 -> coq_Ndouble (coq_lxor p0 q0)
+       | XH -> Npos (XI p0))
+    | XH ->
+      (match q with
+       | XI q0 -> Npos (XO q0)
+       | XO q0 -> Npos (XI q0)
+       | XH -> N0)
+
+  (** val shiftl_nat : positive -> nat -> positive **)
+
+  let shiftl_nat p n0 =
+    nat_iter n0 (fun x -> XO x) p
+
+  (** val shiftr_nat : positive -> nat -> positive **)
+
+  let shiftr_nat p n0 =
+    nat_iter n0 div2 p
+
+  (** val shiftl : positive -> n -> positive **)
+
+  let shiftl p = function
+  | N0 -> p
+  | Npos n1 -> iter n1 (fun x -> XO x) p
+
+  (** val shiftr : positive -> n -> positive **)
+
+  let shiftr p = function
+  | N0 -> p
+  | Npos n1 -> iter n1 div2 p
+
+  (** val testbit_nat : positive -> nat -> bool **)
+
+  let rec testbit_nat p n0 =
+    match p with
+    | XI p0 ->
+      (match n0 with
+       | O -> true
+       | S n' -> testbit_nat p0 n')
+    | XO p0 ->
+      (match n0 with
+       | O -> false
+       | S n' -> testbit_nat p0 n')
+    | XH ->
+      (match n0 with
+       | O -> true
+       | S n1 -> false)
+
+  (** val testbit : positive -> n -> bool **)
+
+  let rec testbit p n0 =
+    match p with
+    | XI p0 ->
+      (match n0 with
+       | N0 -> true
+       | Npos n1 -> testbit p0 (pred_N n1))
+    | XO p0 ->
+      (match n0 with
+       | N0 -> false
+       | Npos n1 -> testbit p0 (pred_N n1))
+    | XH ->
+      (match n0 with
+       | N0 -> true
+       | Npos p0 -> false)
+
+  (** val iter_op : ('a1 -> 'a1 -> 'a1) -> positive -> 'a1 -> 'a1 **)
+
+  let rec iter_op op p a =
+    match p with
+    | XI p0 -> op a (iter_op op p0 (op a a))
+    | XO p0 -> iter_op op p0 (op a a)
+    | XH -> a
+
+  (** val to_nat : positive -> nat **)
+
+  let to_nat x =
+    iter_op plus x (S O)
+
+  (** val of_nat : nat -> positive **)
+
+  let rec of_nat = function
+  | O -> XH
+  | S x ->
+    (match x with
+     | O -> XH
+     | S n1 -> succ (of_nat x))
+
+  (** val of_succ_nat : nat -> positive **)
+
+  let rec of_succ_nat = function
+  | O -> XH
+  | S x -> succ (of_succ_nat x)
+ end
+
+module Coq_Pos =
+ struct
+  type t = positive
+
+  (** val succ : positive -> positive **)
+
+  let rec succ = function
+  | XI p -> XO (succ p)
+  | XO p -> XI p
+  | XH -> XO XH
+
+  (** val add : positive -> positive -> positive **)
+
+  let rec add x y =
+    match x with
+    | XI p ->
+      (match y with
+       | XI q -> XO (add_carry p q)
+       | XO q -> XI (add p q)
+       | XH -> XO (succ p))
+    | XO p ->
+      (match y with
+       | XI q -> XI (add p q)
+       | XO q -> XO (add p q)
+       | XH -> XI p)
+    | XH ->
+      (match y with
+       | XI q -> XO (succ q)
+       | XO q -> XI q
+       | XH -> XO XH)
+
+  (** val add_carry : positive -> positive -> positive **)
+
+  and add_carry x y =
+    match x with
+    | XI p ->
+      (match y with
+       | XI q -> XI (add_carry p q)
+       | XO q -> XO (add_carry p q)
+       | XH -> XI (succ p))
+    | XO p ->
+      (match y with
+       | XI q -> XO (add_carry p q)
+       | XO q -> XI (add p q)
+       | XH -> XO (succ p))
+    | XH ->
+      (match y with
+       | XI q -> XI (succ q)
+       | XO q -> XO (succ q)
+       | XH -> XI XH)
+
+  (** val pred_double : positive -> positive **)
+
+  let rec pred_double = function
+  | XI p -> XI (XO p)
+  | XO p -> XI (pred_double p)
+  | XH -> XH
+
+  (** val pred : positive -> positive **)
+
+  let pred = function
+  | XI p -> XO p
+  | XO p -> pred_double p
+  | XH -> XH
+
+  (** val pred_N : positive -> n **)
+
+  let pred_N = function
+  | XI p -> Npos (XO p)
+  | XO p -> Npos (pred_double p)
+  | XH -> N0
+
+  type mask = Pos.mask =
+  | IsNul
+  | IsPos of positive
+  | IsNeg
+
+  (** val mask_rect : 'a1 -> (positive -> 'a1) -> 'a1 -> mask -> 'a1 **)
+
+  let mask_rect f f0 f1 = function
+  | IsNul -> f
+  | IsPos x -> f0 x
+  | IsNeg -> f1
+
+  (** val mask_rec : 'a1 -> (positive -> 'a1) -> 'a1 -> mask -> 'a1 **)
+
+  let mask_rec f f0 f1 = function
+  | IsNul -> f
+  | IsPos x -> f0 x
+  | IsNeg -> f1
+
+  (** val succ_double_mask : mask -> mask **)
+
+  let succ_double_mask = function
+  | IsNul -> IsPos XH
+  | IsPos p -> IsPos (XI p)
+  | IsNeg -> IsNeg
+
+  (** val double_mask : mask -> mask **)
+
+  let double_mask = function
+  | IsPos p -> IsPos (XO p)
+  | x0 -> x0
+
+  (** val double_pred_mask : positive -> mask **)
+
+  let double_pred_mask = function
+  | XI p -> IsPos (XO (XO p))
+  | XO p -> IsPos (XO (pred_double p))
+  | XH -> IsNul
+
+  (** val pred_mask : mask -> mask **)
+
+  let pred_mask = function
+  | IsPos q ->
+    (match q with
+     | XH -> IsNul
+     | _ -> IsPos (pred q))
+  | _ -> IsNeg
+
+  (** val sub_mask : positive -> positive -> mask **)
+
+  let rec sub_mask x y =
+    match x with
+    | XI p ->
+      (match y with
+       | XI q -> double_mask (sub_mask p q)
+       | XO q -> succ_double_mask (sub_mask p q)
+       | XH -> IsPos (XO p))
+    | XO p ->
+      (match y with
+       | XI q -> succ_double_mask (sub_mask_carry p q)
+       | XO q -> double_mask (sub_mask p q)
+       | XH -> IsPos (pred_double p))
+    | XH ->
+      (match y with
+       | XH -> IsNul
+       | _ -> IsNeg)
+
+  (** val sub_mask_carry : positive -> positive -> mask **)
+
+  and sub_mask_carry x y =
+    match x with
+    | XI p ->
+      (match y with
+       | XI q -> succ_double_mask (sub_mask_carry p q)
+       | XO q -> double_mask (sub_mask p q)
+       | XH -> IsPos (pred_double p))
+    | XO p ->
+      (match y with
+       | XI q -> double_mask (sub_mask_carry p q)
+       | XO q -> succ_double_mask (sub_mask_carry p q)
+       | XH -> double_pred_mask p)
+    | XH -> IsNeg
+
+  (** val sub : positive -> positive -> positive **)
+
+  let sub x y =
+    match sub_mask x y with
+    | IsPos z -> z
+    | _ -> XH
+
+  (** val mul : positive -> positive -> positive **)
+
+  let rec mul x y =
+    match x with
+    | XI p -> add y (XO (mul p y))
+    | XO p -> XO (mul p y)
+    | XH -> y
+
+  (** val iter : positive -> ('a1 -> 'a1) -> 'a1 -> 'a1 **)
+
+  let rec iter n0 f x =
+    match n0 with
+    | XI n' -> f (iter n' f (iter n' f x))
+    | XO n' -> iter n' f (iter n' f x)
+    | XH -> f x
+
+  (** val pow : positive -> positive -> positive **)
+
+  let pow x y =
+    iter y (mul x) XH
+
+  (** val square : positive -> positive **)
+
+  let rec square = function
+  | XI p0 -> XI (XO (add (square p0) p0))
+  | XO p0 -> XO (XO (square p0))
+  | XH -> XH
+
+  (** val div2 : positive -> positive **)
+
+  let div2 = function
+  | XI p0 -> p0
+  | XO p0 -> p0
+  | XH -> XH
+
+  (** val div2_up : positive -> positive **)
+
+  let div2_up = function
+  | XI p0 -> succ p0
+  | XO p0 -> p0
+  | XH -> XH
+
+  (** val size_nat : positive -> nat **)
+
+  let rec size_nat = function
+  | XI p0 -> S (size_nat p0)
+  | XO p0 -> S (size_nat p0)
+  | XH -> S O
+
+  (** val size : positive -> positive **)
+
+  let rec size = function
+  | XI p0 -> succ (size p0)
+  | XO p0 -> succ (size p0)
+  | XH -> XH
+
+  (** val compare_cont :
+      positive -> positive -> comparison -> comparison **)
+
+  let rec compare_cont x y r =
+    match x with
+    | XI p ->
+      (match y with
+       | XI q -> compare_cont p q r
+       | XO q -> compare_cont p q Gt
+       | XH -> Gt)
+    | XO p ->
+      (match y with
+       | XI q -> compare_cont p q Lt
+       | XO q -> compare_cont p q r
+       | XH -> Gt)
+    | XH ->
+      (match y with
+       | XH -> r
+       | _ -> Lt)
+
+  (** val compare : positive -> positive -> comparison **)
+
+  let compare x y =
+    compare_cont x y Eq
+
+  (** val min : positive -> positive -> positive **)
+
+  let min p p' =
+    match compare p p' with
+    | Gt -> p'
+    | _ -> p
+
+  (** val max : positive -> positive -> positive **)
+
+  let max p p' =
+    match compare p p' with
+    | Gt -> p
+    | _ -> p'
+
+  (** val eqb : positive -> positive -> bool **)
+
+  let rec eqb p q =
+    match p with
+    | XI p0 ->
+      (match q with
+       | XI q0 -> eqb p0 q0
+       | _ -> false)
+    | XO p0 ->
+      (match q with
+       | XO q0 -> eqb p0 q0
+       | _ -> false)
+    | XH ->
+      (match q with
+       | XH -> true
+       | _ -> false)
+
+  (** val leb : positive -> positive -> bool **)
+
+  let leb x y =
+    match compare x y with
+    | Gt -> false
+    | _ -> true
+
+  (** val ltb : positive -> positive -> bool **)
+
+  let ltb x y =
+    match compare x y with
+    | Lt -> true
+    | _ -> false
+
+  (** val sqrtrem_step :
+      (positive -> positive) -> (positive -> positive) -> (positive*mask)
+      -> positive*mask **)
+
+  let sqrtrem_step f g = function
+  | s,y ->
+    (match y with
+     | IsPos r ->
+       let s' = XI (XO s) in
+       let r' = g (f r) in
+       if leb s' r' then (XI s),(sub_mask r' s') else (XO s),(IsPos r')
+     | _ -> (XO s),(sub_mask (g (f XH)) (XO (XO XH))))
+
+  (** val sqrtrem : positive -> positive*mask **)
+
+  let rec sqrtrem = function
+  | XI p0 ->
+    (match p0 with
+     | XI p1 -> sqrtrem_step (fun x -> XI x) (fun x -> XI x) (sqrtrem p1)
+     | XO p1 -> sqrtrem_step (fun x -> XO x) (fun x -> XI x) (sqrtrem p1)
+     | XH -> XH,(IsPos (XO XH)))
+  | XO p0 ->
+    (match p0 with
+     | XI p1 -> sqrtrem_step (fun x -> XI x) (fun x -> XO x) (sqrtrem p1)
+     | XO p1 -> sqrtrem_step (fun x -> XO x) (fun x -> XO x) (sqrtrem p1)
+     | XH -> XH,(IsPos XH))
+  | XH -> XH,IsNul
+
+  (** val sqrt : positive -> positive **)
+
+  let sqrt p =
+    fst (sqrtrem p)
+
+  (** val gcdn : nat -> positive -> positive -> positive **)
+
+  let rec gcdn n0 a b =
+    match n0 with
+    | O -> XH
+    | S n1 ->
+      (match a with
+       | XI a' ->
+         (match b with
+          | XI b' ->
+            (match compare a' b' with
+             | Eq -> a
+             | Lt -> gcdn n1 (sub b' a') a
+             | Gt -> gcdn n1 (sub a' b') b)
+          | XO b0 -> gcdn n1 a b0
+          | XH -> XH)
+       | XO a0 ->
+         (match b with
+          | XI p -> gcdn n1 a0 b
+          | XO b0 -> XO (gcdn n1 a0 b0)
+          | XH -> XH)
+       | XH -> XH)
+
+  (** val gcd : positive -> positive -> positive **)
+
+  let gcd a b =
+    gcdn (plus (size_nat a) (size_nat b)) a b
+
+  (** val ggcdn :
+      nat -> positive -> positive -> positive*(positive*positive) **)
+
+  let rec ggcdn n0 a b =
+    match n0 with
+    | O -> XH,(a,b)
+    | S n1 ->
+      (match a with
+       | XI a' ->
+         (match b with
+          | XI b' ->
+            (match compare a' b' with
+             | Eq -> a,(XH,XH)
+             | Lt ->
+               let g,p = ggcdn n1 (sub b' a') a in
+               let ba,aa = p in g,(aa,(add aa (XO ba)))
+             | Gt ->
+               let g,p = ggcdn n1 (sub a' b') b in
+               let ab,bb = p in g,((add bb (XO ab)),bb))
+          | XO b0 ->
+            let g,p = ggcdn n1 a b0 in let aa,bb = p in g,(aa,(XO bb))
+          | XH -> XH,(a,XH))
+       | XO a0 ->
+         (match b with
+          | XI p ->
+            let g,p0 = ggcdn n1 a0 b in let aa,bb = p0 in g,((XO aa),bb)
+          | XO b0 -> let g,p = ggcdn n1 a0 b0 in (XO g),p
+          | XH -> XH,(a,XH))
+       | XH -> XH,(XH,b))
+
+  (** val ggcd : positive -> positive -> positive*(positive*positive) **)
+
+  let ggcd a b =
+    ggcdn (plus (size_nat a) (size_nat b)) a b
+
+  (** val coq_Nsucc_double : n -> n **)
+
+  let coq_Nsucc_double = function
+  | N0 -> Npos XH
+  | Npos p -> Npos (XI p)
+
+  (** val coq_Ndouble : n -> n **)
+
+  let coq_Ndouble = function
+  | N0 -> N0
+  | Npos p -> Npos (XO p)
+
+  (** val coq_lor : positive -> positive -> positive **)
+
+  let rec coq_lor p q =
+    match p with
+    | XI p0 ->
+      (match q with
+       | XI q0 -> XI (coq_lor p0 q0)
+       | XO q0 -> XI (coq_lor p0 q0)
+       | XH -> p)
+    | XO p0 ->
+      (match q with
+       | XI q0 -> XI (coq_lor p0 q0)
+       | XO q0 -> XO (coq_lor p0 q0)
+       | XH -> XI p0)
+    | XH ->
+      (match q with
+       | XO q0 -> XI q0
+       | _ -> q)
+
+  (** val coq_land : positive -> positive -> n **)
+
+  let rec coq_land p q =
+    match p with
+    | XI p0 ->
+      (match q with
+       | XI q0 -> coq_Nsucc_double (coq_land p0 q0)
+       | XO q0 -> coq_Ndouble (coq_land p0 q0)
+       | XH -> Npos XH)
+    | XO p0 ->
+      (match q with
+       | XI q0 -> coq_Ndouble (coq_land p0 q0)
+       | XO q0 -> coq_Ndouble (coq_land p0 q0)
+       | XH -> N0)
+    | XH ->
+      (match q with
+       | XO q0 -> N0
+       | _ -> Npos XH)
+
+  (** val ldiff : positive -> positive -> n **)
+
+  let rec ldiff p q =
+    match p with
+    | XI p0 ->
+      (match q with
+       | XI q0 -> coq_Ndouble (ldiff p0 q0)
+       | XO q0 -> coq_Nsucc_double (ldiff p0 q0)
+       | XH -> Npos (XO p0))
+    | XO p0 ->
+      (match q with
+       | XI q0 -> coq_Ndouble (ldiff p0 q0)
+       | XO q0 -> coq_Ndouble (ldiff p0 q0)
+       | XH -> Npos p)
+    | XH ->
+      (match q with
+       | XO q0 -> Npos XH
+       | _ -> N0)
+
+  (** val coq_lxor : positive -> positive -> n **)
+
+  let rec coq_lxor p q =
+    match p with
+    | XI p0 ->
+      (match q with
+       | XI q0 -> coq_Ndouble (coq_lxor p0 q0)
+       | XO q0 -> coq_Nsucc_double (coq_lxor p0 q0)
+       | XH -> Npos (XO p0))
+    | XO p0 ->
+      (match q with
+       | XI q0 -> coq_Nsucc_double (coq_lxor p0 q0)
+       | XO q0 -> coq_Ndouble (coq_lxor p0 q0)
+       | XH -> Npos (XI p0))
+    | XH ->
+      (match q with
+       | XI q0 -> Npos (XO q0)
+       | XO q0 -> Npos (XI q0)
+       | XH -> N0)
+
+  (** val shiftl_nat : positive -> nat -> positive **)
+
+  let shiftl_nat p n0 =
+    nat_iter n0 (fun x -> XO x) p
+
+  (** val shiftr_nat : positive -> nat -> positive **)
+
+  let shiftr_nat p n0 =
+    nat_iter n0 div2 p
+
+  (** val shiftl : positive -> n -> positive **)
+
+  let shiftl p = function
+  | N0 -> p
+  | Npos n1 -> iter n1 (fun x -> XO x) p
+
+  (** val shiftr : positive -> n -> positive **)
+
+  let shiftr p = function
+  | N0 -> p
+  | Npos n1 -> iter n1 div2 p
+
+  (** val testbit_nat : positive -> nat -> bool **)
+
+  let rec testbit_nat p n0 =
+    match p with
+    | XI p0 ->
+      (match n0 with
+       | O -> true
+       | S n' -> testbit_nat p0 n')
+    | XO p0 ->
+      (match n0 with
+       | O -> false
+       | S n' -> testbit_nat p0 n')
+    | XH ->
+      (match n0 with
+       | O -> true
+       | S n1 -> false)
+
+  (** val testbit : positive -> n -> bool **)
+
+  let rec testbit p n0 =
+    match p with
+    | XI p0 ->
+      (match n0 with
+       | N0 -> true
+       | Npos n1 -> testbit p0 (pred_N n1))
+    | XO p0 ->
+      (match n0 with
+       | N0 -> false
+       | Npos n1 -> testbit p0 (pred_N n1))
+    | XH ->
+      (match n0 with
+       | N0 -> true
+       | Npos p0 -> false)
+
+  (** val iter_op : ('a1 -> 'a1 -> 'a1) -> positive -> 'a1 -> 'a1 **)
+
+  let rec iter_op op p a =
+    match p with
+    | XI p0 -> op a (iter_op op p0 (op a a))
+    | XO p0 -> iter_op op p0 (op a a)
+    | XH -> a
+
+  (** val to_nat : positive -> nat **)
+
+  let to_nat x =
+    iter_op plus x (S O)
+
+  (** val of_nat : nat -> positive **)
+
+  let rec of_nat = function
+  | O -> XH
+  | S x ->
+    (match x with
+     | O -> XH
+     | S n1 -> succ (of_nat x))
+
+  (** val of_succ_nat : nat -> positive **)
+
+  let rec of_succ_nat = function
+  | O -> XH
+  | S x -> succ (of_succ_nat x)
+
+  (** val eq_dec : positive -> positive -> bool **)
+
+  let rec eq_dec p y0 =
+    match p with
+    | XI p0 ->
+      (match y0 with
+       | XI p1 -> eq_dec p0 p1
+       | _ -> false)
+    | XO p0 ->
+      (match y0 with
+       | XO p1 -> eq_dec p0 p1
+       | _ -> false)
+    | XH ->
+      (match y0 with
+       | XH -> true
+       | _ -> false)
+
+  (** val peano_rect :
+      'a1 -> (positive -> 'a1 -> 'a1) -> positive -> 'a1 **)
+
+  let rec peano_rect a f p =
+    let f2 =
+      peano_rect (f XH a) (fun p0 x -> f (succ (XO p0)) (f (XO p0) x))
+    in
+    (match p with
+     | XI q -> f (XO q) (f2 q)
+     | XO q -> f2 q
+     | XH -> a)
+
+  (** val peano_rec :
+      'a1 -> (positive -> 'a1 -> 'a1) -> positive -> 'a1 **)
+
+  let peano_rec =
+    peano_rect
+
+  type coq_PeanoView =
+  | PeanoOne
+  | PeanoSucc of positive * coq_PeanoView
+
+  (** val coq_PeanoView_rect :
+      'a1 -> (positive -> coq_PeanoView -> 'a1 -> 'a1) -> positive ->
+      coq_PeanoView -> 'a1 **)
+
+  let rec coq_PeanoView_rect f f0 p = function
+  | PeanoOne -> f
+  | PeanoSucc (p1, p2) -> f0 p1 p2 (coq_PeanoView_rect f f0 p1 p2)
+
+  (** val coq_PeanoView_rec :
+      'a1 -> (positive -> coq_PeanoView -> 'a1 -> 'a1) -> positive ->
+      coq_PeanoView -> 'a1 **)
+
+  let rec coq_PeanoView_rec f f0 p = function
+  | PeanoOne -> f
+  | PeanoSucc (p1, p2) -> f0 p1 p2 (coq_PeanoView_rec f f0 p1 p2)
+
+  (** val peanoView_xO : positive -> coq_PeanoView -> coq_PeanoView **)
+
+  let rec peanoView_xO p = function
+  | PeanoOne -> PeanoSucc (XH, PeanoOne)
+  | PeanoSucc (p0, q0) ->
+    PeanoSucc ((succ (XO p0)), (PeanoSucc ((XO p0),
+      (peanoView_xO p0 q0))))
+
+  (** val peanoView_xI : positive -> coq_PeanoView -> coq_PeanoView **)
+
+  let rec peanoView_xI p = function
+  | PeanoOne -> PeanoSucc ((succ XH), (PeanoSucc (XH, PeanoOne)))
+  | PeanoSucc (p0, q0) ->
+    PeanoSucc ((succ (XI p0)), (PeanoSucc ((XI p0),
+      (peanoView_xI p0 q0))))
+
+  (** val peanoView : positive -> coq_PeanoView **)
+
+  let rec peanoView = function
+  | XI p0 -> peanoView_xI p0 (peanoView p0)
+  | XO p0 -> peanoView_xO p0 (peanoView p0)
+  | XH -> PeanoOne
+
+  (** val coq_PeanoView_iter :
+      'a1 -> (positive -> 'a1 -> 'a1) -> positive -> coq_PeanoView -> 'a1 **)
+
+  let rec coq_PeanoView_iter a f p = function
+  | PeanoOne -> a
+  | PeanoSucc (p0, q0) -> f p0 (coq_PeanoView_iter a f p0 q0)
+
+  (** val eqb_spec : positive -> positive -> reflect **)
+
+  let eqb_spec x y =
+    iff_reflect (eqb x y)
+
+  (** val switch_Eq : comparison -> comparison -> comparison **)
+
+  let switch_Eq c = function
+  | Eq -> c
+  | x -> x
+
+  (** val mask2cmp : mask -> comparison **)
+
+  let mask2cmp = function
+  | IsNul -> Eq
+  | IsPos p0 -> Gt
+  | IsNeg -> Lt
+
+  (** val leb_spec0 : positive -> positive -> reflect **)
+
+  let leb_spec0 x y =
+    iff_reflect (leb x y)
+
+  (** val ltb_spec0 : positive -> positive -> reflect **)
+
+  let ltb_spec0 x y =
+    iff_reflect (ltb x y)
+
+  module Private_Tac =
+   struct
+
+   end
+
+  module Private_Dec =
+   struct
+    (** val max_case_strong :
+        positive -> positive -> (positive -> positive -> __ -> 'a1 -> 'a1)
+        -> (__ -> 'a1) -> (__ -> 'a1) -> 'a1 **)
+
+    let max_case_strong n0 m compat hl hr =
+      let c = compSpec2Type n0 m (compare n0 m) in
+      (match c with
+       | CompGtT -> compat n0 (max n0 m) __ (hl __)
+       | _ -> compat m (max n0 m) __ (hr __))
+
+    (** val max_case :
+        positive -> positive -> (positive -> positive -> __ -> 'a1 -> 'a1)
+        -> 'a1 -> 'a1 -> 'a1 **)
+
+    let max_case n0 m x x0 x1 =
+      max_case_strong n0 m x (fun _ -> x0) (fun _ -> x1)
+
+    (** val max_dec : positive -> positive -> bool **)
+
+    let max_dec n0 m =
+      max_case n0 m (fun x y _ h0 -> h0) true false
+
+    (** val min_case_strong :
+        positive -> positive -> (positive -> positive -> __ -> 'a1 -> 'a1)
+        -> (__ -> 'a1) -> (__ -> 'a1) -> 'a1 **)
+
+    let min_case_strong n0 m compat hl hr =
+      let c = compSpec2Type n0 m (compare n0 m) in
+      (match c with
+       | CompGtT -> compat m (min n0 m) __ (hr __)
+       | _ -> compat n0 (min n0 m) __ (hl __))
+
+    (** val min_case :
+        positive -> positive -> (positive -> positive -> __ -> 'a1 -> 'a1)
+        -> 'a1 -> 'a1 -> 'a1 **)
+
+    let min_case n0 m x x0 x1 =
+      min_case_strong n0 m x (fun _ -> x0) (fun _ -> x1)
+
+    (** val min_dec : positive -> positive -> bool **)
+
+    let min_dec n0 m =
+      min_case n0 m (fun x y _ h0 -> h0) true false
+   end
+
+  (** val max_case_strong :
+      positive -> positive -> (__ -> 'a1) -> (__ -> 'a1) -> 'a1 **)
+
+  let max_case_strong n0 m x x0 =
+    Private_Dec.max_case_strong n0 m (fun x1 y _ x2 -> x2) x x0
+
+  (** val max_case : positive -> positive -> 'a1 -> 'a1 -> 'a1 **)
+
+  let max_case n0 m x x0 =
+    max_case_strong n0 m (fun _ -> x) (fun _ -> x0)
+
+  (** val max_dec : positive -> positive -> bool **)
+
+  let max_dec =
+    Private_Dec.max_dec
+
+  (** val min_case_strong :
+      positive -> positive -> (__ -> 'a1) -> (__ -> 'a1) -> 'a1 **)
+
+  let min_case_strong n0 m x x0 =
+    Private_Dec.min_case_strong n0 m (fun x1 y _ x2 -> x2) x x0
+
+  (** val min_case : positive -> positive -> 'a1 -> 'a1 -> 'a1 **)
+
+  let min_case n0 m x x0 =
+    min_case_strong n0 m (fun _ -> x) (fun _ -> x0)
+
+  (** val min_dec : positive -> positive -> bool **)
+
+  let min_dec =
+    Private_Dec.min_dec
+ end
+
+module N =
+ struct
+  type t = n
+
+  (** val zero : n **)
+
+  let zero =
+    N0
+
+  (** val one : n **)
+
+  let one =
+    Npos XH
+
+  (** val two : n **)
+
+  let two =
+    Npos (XO XH)
+
+  (** val succ_double : n -> n **)
+
+  let succ_double = function
+  | N0 -> Npos XH
+  | Npos p -> Npos (XI p)
+
+  (** val double : n -> n **)
+
+  let double = function
+  | N0 -> N0
+  | Npos p -> Npos (XO p)
+
+  (** val succ : n -> n **)
+
+  let succ = function
+  | N0 -> Npos XH
+  | Npos p -> Npos (Coq_Pos.succ p)
+
+  (** val pred : n -> n **)
+
+  let pred = function
+  | N0 -> N0
+  | Npos p -> Coq_Pos.pred_N p
+
+  (** val succ_pos : n -> positive **)
+
+  let succ_pos = function
+  | N0 -> XH
+  | Npos p -> Coq_Pos.succ p
+
+  (** val add : n -> n -> n **)
+
+  let add n0 m =
+    match n0 with
+    | N0 -> m
+    | Npos p ->
+      (match m with
+       | N0 -> n0
+       | Npos q -> Npos (Coq_Pos.add p q))
+
+  (** val sub : n -> n -> n **)
+
+  let sub n0 m =
+    match n0 with
+    | N0 -> N0
+    | Npos n' ->
+      (match m with
+       | N0 -> n0
+       | Npos m' ->
+         (match Coq_Pos.sub_mask n' m' with
+          | Coq_Pos.IsPos p -> Npos p
+          | _ -> N0))
+
+  (** val mul : n -> n -> n **)
+
+  let mul n0 m =
+    match n0 with
+    | N0 -> N0
+    | Npos p ->
+      (match m with
+       | N0 -> N0
+       | Npos q -> Npos (Coq_Pos.mul p q))
+
+  (** val compare : n -> n -> comparison **)
+
+  let compare n0 m =
+    match n0 with
+    | N0 ->
+      (match m with
+       | N0 -> Eq
+       | Npos m' -> Lt)
+    | Npos n' ->
+      (match m with
+       | N0 -> Gt
+       | Npos m' -> Coq_Pos.compare n' m')
+
+  (** val eqb : n -> n -> bool **)
+
+  let rec eqb n0 m =
+    match n0 with
+    | N0 ->
+      (match m with
+       | N0 -> true
+       | Npos p -> false)
+    | Npos p ->
+      (match m with
+       | N0 -> false
+       | Npos q -> Coq_Pos.eqb p q)
+
+  (** val leb : n -> n -> bool **)
+
+  let leb x y =
+    match compare x y with
+    | Gt -> false
+    | _ -> true
+
+  (** val ltb : n -> n -> bool **)
+
+  let ltb x y =
+    match compare x y with
+    | Lt -> true
+    | _ -> false
+
+  (** val min : n -> n -> n **)
+
+  let min n0 n' =
+    match compare n0 n' with
+    | Gt -> n'
+    | _ -> n0
+
+  (** val max : n -> n -> n **)
+
+  let max n0 n' =
+    match compare n0 n' with
+    | Gt -> n0
+    | _ -> n'
+
+  (** val div2 : n -> n **)
+
+  let div2 = function
+  | N0 -> N0
+  | Npos p0 ->
+    (match p0 with
+     | XI p -> Npos p
+     | XO p -> Npos p
+     | XH -> N0)
+
+  (** val even : n -> bool **)
+
+  let even = function
+  | N0 -> true
+  | Npos p ->
+    (match p with
+     | XO p0 -> true
+     | _ -> false)
+
+  (** val odd : n -> bool **)
+
+  let odd n0 =
+    negb (even n0)
+
+  (** val pow : n -> n -> n **)
+
+  let pow n0 = function
+  | N0 -> Npos XH
+  | Npos p0 ->
+    (match n0 with
+     | N0 -> N0
+     | Npos q -> Npos (Coq_Pos.pow q p0))
+
+  (** val square : n -> n **)
+
+  let square = function
+  | N0 -> N0
+  | Npos p -> Npos (Coq_Pos.square p)
+
+  (** val log2 : n -> n **)
+
+  let log2 = function
+  | N0 -> N0
+  | Npos p0 ->
+    (match p0 with
+     | XI p -> Npos (Coq_Pos.size p)
+     | XO p -> Npos (Coq_Pos.size p)
+     | XH -> N0)
+
+  (** val size : n -> n **)
+
+  let size = function
+  | N0 -> N0
+  | Npos p -> Npos (Coq_Pos.size p)
+
+  (** val size_nat : n -> nat **)
+
+  let size_nat = function
+  | N0 -> O
+  | Npos p -> Coq_Pos.size_nat p
+
+  (** val pos_div_eucl : positive -> n -> n*n **)
+
+  let rec pos_div_eucl a b =
+    match a with
+    | XI a' ->
+      let q,r = pos_div_eucl a' b in
+      let r' = succ_double r in
+      if leb b r' then (succ_double q),(sub r' b) else (double q),r'
+    | XO a' ->
+      let q,r = pos_div_eucl a' b in
+      let r' = double r in
+      if leb b r' then (succ_double q),(sub r' b) else (double q),r'
+    | XH ->
+      (match b with
+       | N0 -> N0,(Npos XH)
+       | Npos p ->
+         (match p with
+          | XH -> (Npos XH),N0
+          | _ -> N0,(Npos XH)))
+
+  (** val div_eucl : n -> n -> n*n **)
+
+  let div_eucl a b =
+    match a with
+    | N0 -> N0,N0
+    | Npos na ->
+      (match b with
+       | N0 -> N0,a
+       | Npos p -> pos_div_eucl na b)
+
+  (** val div : n -> n -> n **)
+
+  let div a b =
+    fst (div_eucl a b)
+
+  (** val modulo : n -> n -> n **)
+
+  let modulo a b =
+    snd (div_eucl a b)
+
+  (** val gcd : n -> n -> n **)
+
+  let gcd a b =
+    match a with
+    | N0 -> b
+    | Npos p ->
+      (match b with
+       | N0 -> a
+       | Npos q -> Npos (Coq_Pos.gcd p q))
+
+  (** val ggcd : n -> n -> n*(n*n) **)
+
+  let ggcd a b =
+    match a with
+    | N0 -> b,(N0,(Npos XH))
+    | Npos p ->
+      (match b with
+       | N0 -> a,((Npos XH),N0)
+       | Npos q ->
+         let g,p0 = Coq_Pos.ggcd p q in
+         let aa,bb = p0 in (Npos g),((Npos aa),(Npos bb)))
+
+  (** val sqrtrem : n -> n*n **)
+
+  let sqrtrem = function
+  | N0 -> N0,N0
+  | Npos p ->
+    let s,m = Coq_Pos.sqrtrem p in
+    (match m with
+     | Coq_Pos.IsPos r -> (Npos s),(Npos r)
+     | _ -> (Npos s),N0)
+
+  (** val sqrt : n -> n **)
+
+  let sqrt = function
+  | N0 -> N0
+  | Npos p -> Npos (Coq_Pos.sqrt p)
+
+  (** val coq_lor : n -> n -> n **)
+
+  let coq_lor n0 m =
+    match n0 with
+    | N0 -> m
+    | Npos p ->
+      (match m with
+       | N0 -> n0
+       | Npos q -> Npos (Coq_Pos.coq_lor p q))
+
+  (** val coq_land : n -> n -> n **)
+
+  let coq_land n0 m =
+    match n0 with
+    | N0 -> N0
+    | Npos p ->
+      (match m with
+       | N0 -> N0
+       | Npos q -> Coq_Pos.coq_land p q)
+
+  (** val ldiff : n -> n -> n **)
+
+  let rec ldiff n0 m =
+    match n0 with
+    | N0 -> N0
+    | Npos p ->
+      (match m with
+       | N0 -> n0
+       | Npos q -> Coq_Pos.ldiff p q)
+
+  (** val coq_lxor : n -> n -> n **)
+
+  let coq_lxor n0 m =
+    match n0 with
+    | N0 -> m
+    | Npos p ->
+      (match m with
+       | N0 -> n0
+       | Npos q -> Coq_Pos.coq_lxor p q)
+
+  (** val shiftl_nat : n -> nat -> n **)
+
+  let shiftl_nat a n0 =
+    nat_iter n0 double a
+
+  (** val shiftr_nat : n -> nat -> n **)
+
+  let shiftr_nat a n0 =
+    nat_iter n0 div2 a
+
+  (** val shiftl : n -> n -> n **)
+
+  let shiftl a n0 =
+    match a with
+    | N0 -> N0
+    | Npos a0 -> Npos (Coq_Pos.shiftl a0 n0)
+
+  (** val shiftr : n -> n -> n **)
+
+  let shiftr a = function
+  | N0 -> a
+  | Npos p -> Coq_Pos.iter p div2 a
+
+  (** val testbit_nat : n -> nat -> bool **)
+
+  let testbit_nat = function
+  | N0 -> (fun x -> false)
+  | Npos p -> Coq_Pos.testbit_nat p
+
+  (** val testbit : n -> n -> bool **)
+
+  let testbit a n0 =
+    match a with
+    | N0 -> false
+    | Npos p -> Coq_Pos.testbit p n0
+
+  (** val to_nat : n -> nat **)
+
+  let to_nat = function
+  | N0 -> O
+  | Npos p -> Coq_Pos.to_nat p
+
+  (** val of_nat : nat -> n **)
+
+  let of_nat = function
+  | O -> N0
+  | S n' -> Npos (Coq_Pos.of_succ_nat n')
+
+  (** val iter : n -> ('a1 -> 'a1) -> 'a1 -> 'a1 **)
+
+  let iter n0 f x =
+    match n0 with
+    | N0 -> x
+    | Npos p -> Coq_Pos.iter p f x
+
+  (** val eq_dec : n -> n -> bool **)
+
+  let eq_dec n0 m =
+    match n0 with
+    | N0 ->
+      (match m with
+       | N0 -> true
+       | Npos p -> false)
+    | Npos x ->
+      (match m with
+       | N0 -> false
+       | Npos p0 -> Coq_Pos.eq_dec x p0)
+
+  (** val discr : n -> positive sumor **)
+
+  let discr = function
+  | N0 -> Inright
+  | Npos p -> Inleft p
+
+  (** val binary_rect :
+      'a1 -> (n -> 'a1 -> 'a1) -> (n -> 'a1 -> 'a1) -> n -> 'a1 **)
+
+  let binary_rect f0 f2 fS2 n0 =
+    let f2' = fun p -> f2 (Npos p) in
+    let fS2' = fun p -> fS2 (Npos p) in
+    (match n0 with
+     | N0 -> f0
+     | Npos p ->
+       let rec f = function
+       | XI p1 -> fS2' p1 (f p1)
+       | XO p1 -> f2' p1 (f p1)
+       | XH -> fS2 N0 f0
+       in f p)
+
+  (** val binary_rec :
+      'a1 -> (n -> 'a1 -> 'a1) -> (n -> 'a1 -> 'a1) -> n -> 'a1 **)
+
+  let binary_rec =
+    binary_rect
+
+  (** val peano_rect : 'a1 -> (n -> 'a1 -> 'a1) -> n -> 'a1 **)
+
+  let peano_rect f0 f n0 =
+    let f' = fun p -> f (Npos p) in
+    (match n0 with
+     | N0 -> f0
+     | Npos p -> Coq_Pos.peano_rect (f N0 f0) f' p)
+
+  (** val peano_rec : 'a1 -> (n -> 'a1 -> 'a1) -> n -> 'a1 **)
+
+  let peano_rec =
+    peano_rect
+
+  (** val leb_spec0 : n -> n -> reflect **)
+
+  let leb_spec0 x y =
+    iff_reflect (leb x y)
+
+  (** val ltb_spec0 : n -> n -> reflect **)
+
+  let ltb_spec0 x y =
+    iff_reflect (ltb x y)
+
+  module Private_BootStrap =
+   struct
+
+   end
+
+  (** val recursion : 'a1 -> (n -> 'a1 -> 'a1) -> n -> 'a1 **)
+
+  let recursion x =
+    peano_rect x
+
+  module Private_OrderTac =
+   struct
+    module IsTotal =
+     struct
+
+     end
+
+    module Tac =
+     struct
+
+     end
+   end
+
+  module Private_NZPow =
+   struct
+
+   end
+
+  module Private_NZSqrt =
+   struct
+
+   end
+
+  (** val sqrt_up : n -> n **)
+
+  let sqrt_up a =
+    match compare N0 a with
+    | Lt -> succ (sqrt (pred a))
+    | _ -> N0
+
+  (** val log2_up : n -> n **)
+
+  let log2_up a =
+    match compare (Npos XH) a with
+    | Lt -> succ (log2 (pred a))
+    | _ -> N0
+
+  module Private_NZDiv =
+   struct
+
+   end
+
+  (** val lcm : n -> n -> n **)
+
+  let lcm a b =
+    mul a (div b (gcd a b))
+
+  (** val eqb_spec : n -> n -> reflect **)
+
+  let eqb_spec x y =
+    iff_reflect (eqb x y)
+
+  (** val b2n : bool -> n **)
+
+  let b2n = function
+  | true -> Npos XH
+  | false -> N0
+
+  (** val setbit : n -> n -> n **)
+
+  let setbit a n0 =
+    coq_lor a (shiftl (Npos XH) n0)
+
+  (** val clearbit : n -> n -> n **)
+
+  let clearbit a n0 =
+    ldiff a (shiftl (Npos XH) n0)
+
+  (** val ones : n -> n **)
+
+  let ones n0 =
+    pred (shiftl (Npos XH) n0)
+
+  (** val lnot : n -> n -> n **)
+
+  let lnot a n0 =
+    coq_lxor a (ones n0)
+
+  module Private_Tac =
+   struct
+
+   end
+
+  module Private_Dec =
+   struct
+    (** val max_case_strong :
+        n -> n -> (n -> n -> __ -> 'a1 -> 'a1) -> (__ -> 'a1) -> (__ ->
+        'a1) -> 'a1 **)
+
+    let max_case_strong n0 m compat hl hr =
+      let c = compSpec2Type n0 m (compare n0 m) in
+      (match c with
+       | CompGtT -> compat n0 (max n0 m) __ (hl __)
+       | _ -> compat m (max n0 m) __ (hr __))
+
+    (** val max_case :
+        n -> n -> (n -> n -> __ -> 'a1 -> 'a1) -> 'a1 -> 'a1 -> 'a1 **)
+
+    let max_case n0 m x x0 x1 =
+      max_case_strong n0 m x (fun _ -> x0) (fun _ -> x1)
+
+    (** val max_dec : n -> n -> bool **)
+
+    let max_dec n0 m =
+      max_case n0 m (fun x y _ h0 -> h0) true false
+
+    (** val min_case_strong :
+        n -> n -> (n -> n -> __ -> 'a1 -> 'a1) -> (__ -> 'a1) -> (__ ->
+        'a1) -> 'a1 **)
+
+    let min_case_strong n0 m compat hl hr =
+      let c = compSpec2Type n0 m (compare n0 m) in
+      (match c with
+       | CompGtT -> compat m (min n0 m) __ (hr __)
+       | _ -> compat n0 (min n0 m) __ (hl __))
+
+    (** val min_case :
+        n -> n -> (n -> n -> __ -> 'a1 -> 'a1) -> 'a1 -> 'a1 -> 'a1 **)
+
+    let min_case n0 m x x0 x1 =
+      min_case_strong n0 m x (fun _ -> x0) (fun _ -> x1)
+
+    (** val min_dec : n -> n -> bool **)
+
+    let min_dec n0 m =
+      min_case n0 m (fun x y _ h0 -> h0) true false
+   end
+
+  (** val max_case_strong :
+      n -> n -> (__ -> 'a1) -> (__ -> 'a1) -> 'a1 **)
+
+  let max_case_strong n0 m x x0 =
+    Private_Dec.max_case_strong n0 m (fun x1 y _ x2 -> x2) x x0
+
+  (** val max_case : n -> n -> 'a1 -> 'a1 -> 'a1 **)
+
+  let max_case n0 m x x0 =
+    max_case_strong n0 m (fun _ -> x) (fun _ -> x0)
+
+  (** val max_dec : n -> n -> bool **)
+
+  let max_dec =
+    Private_Dec.max_dec
+
+  (** val min_case_strong :
+      n -> n -> (__ -> 'a1) -> (__ -> 'a1) -> 'a1 **)
+
+  let min_case_strong n0 m x x0 =
+    Private_Dec.min_case_strong n0 m (fun x1 y _ x2 -> x2) x x0
+
+  (** val min_case : n -> n -> 'a1 -> 'a1 -> 'a1 **)
+
+  let min_case n0 m x x0 =
+    min_case_strong n0 m (fun _ -> x) (fun _ -> x0)
+
+  (** val min_dec : n -> n -> bool **)
+
+  let min_dec =
+    Private_Dec.min_dec
+ end
+
+(** val exp2' : nat -> positive **)
+
+let rec exp2' = function
+| O -> XH
+| S l' -> XO (exp2' l')
+
+(** val exp2 : nat -> n **)
+
+let exp2 l =
+  Npos (exp2' l)
+
+(** val exp2_nat : nat -> nat **)
+
+let exp2_nat l =
+  N.to_nat (exp2 l)
+
+(** val encode'' : positive -> bin_t -> bool list **)
+
+let rec encode'' pos acc =
+  match pos with
+  | XI pos' -> encode'' pos' (true::acc)
+  | XO pos' -> encode'' pos' (false::acc)
+  | XH -> true::acc
+
+(** val encode' : n -> bool list **)
+
+let encode' = function
+| N0 -> []
+| Npos pos -> encode'' pos []
+
+(** val pad : bin_t -> nat -> bin_t **)
+
+let rec pad b = function
+| O -> b
+| S l' -> false::(pad b l')
+
+(** val fixInt_encode : nat -> n -> bin_t **)
+
+let fixInt_encode size0 n0 =
+  let b = encode' n0 in pad b (minus size0 (length b))
+
+(** val decode'' : bin_t -> nat -> positive -> positive*bin_t **)
+
+let rec decode'' b l acc =
+  match l with
+  | O -> acc,b
+  | S l' ->
+    (match b with
+     | [] -> acc,[]
+     | b0::b' ->
+       if b0 then decode'' b' l' (XI acc) else decode'' b' l' (XO acc))
+
+(** val decode' : bin_t -> nat -> n*bin_t **)
+
+let rec decode' b = function
+| O -> N0,b
+| S l' ->
+  (match b with
+   | [] -> N0,[]
+   | b0::b' ->
+     if b0
+     then let pos,b'' = decode'' b' l' XH in (Npos pos),b''
+     else decode' b' l')
+
+(** val fixInt_decode : nat -> bin_t -> n*bin_t **)
+
+let fixInt_decode size0 b =
+  (fst (decode' b size0)),(snd (decode' b size0))
+
+type 'a data_t = 'a list
+
+(** val encode'0 : 'a1 -> (('a1*'a2) -> 'a2) -> 'a1 list -> 'a2 -> 'a2 **)
+
+let rec encode'0 halt0 encode_A data ext =
+  match data with
+  | [] -> encode_A (halt0,ext)
+  | s::data' -> encode_A (s,(encode'0 halt0 encode_A data' ext))
+
+(** val steppingList_encode :
+    'a1 -> nat -> (('a1*'a2) -> 'a2) -> ('a1 data_t*'a2) -> 'a2 **)
+
+let steppingList_encode halt0 fuel encode_A = function
+| _a,_bin -> encode'0 halt0 encode_A _a _bin
+
+(** val decode'0 :
+    'a1 -> ('a1 -> bool) -> (('a1*'a2) -> 'a2) -> ('a1*'a2, 'a2) decoder
+    -> 'a2 -> nat -> 'a1 list*'a2 **)
+
+let rec decode'0 halt0 halt_dec0 encode_A decoder_A b f =
+  let x,b' = decode encode_A decoder_A b in
+  if halt_dec0 x
+  then [],b'
+  else (match f with
+        | O -> [],b'
+        | S f' ->
+          let xs,b'' = decode'0 halt0 halt_dec0 encode_A decoder_A b' f'
+          in
+          (x::xs),b'')
+
+(** val steppingList_decode :
+    'a1 -> ('a1 -> bool) -> nat -> (('a1*'a2) -> 'a2) -> ('a1*'a2, 'a2)
+    decoder -> 'a2 -> 'a1 data_t*'a2 **)
+
+let steppingList_decode halt0 halt_dec0 fuel encode_A decoder_A b =
+  (fst (decode'0 halt0 halt_dec0 encode_A decoder_A b fuel)),(snd
+                                                               (decode'0
+                                                                 halt0
+                                                                 halt_dec0
+                                                                 encode_A
+                                                                 decoder_A
+                                                                 b fuel))
+
+(** val steppingList_decoder :
+    'a1 -> ('a1 -> bool) -> nat -> (('a1*bin_t) -> bin_t) -> ('a1*bin_t,
+    bin_t) decoder -> ('a1 data_t*bin_t, bin_t) decoder **)
+
+let steppingList_decoder halt0 halt_dec0 fuel encode_A decoder_A =
+  steppingList_decode halt0 halt_dec0 fuel encode_A decoder_A
+
+type 'a data_t0 = 'a list
+
+(** val fixList_getlength : nat -> 'a1 data_t0 -> n **)
+
+let fixList_getlength size0 ls =
+  N.of_nat (length ls)
+
+(** val encode'1 : (('a1*'a2) -> 'a2) -> 'a1 list -> 'a2 -> 'a2 **)
+
+let rec encode'1 encode_A xs ext =
+  match xs with
+  | [] -> ext
+  | x::xs0 -> encode_A (x,(encode'1 encode_A xs0 ext))
+
+(** val fixList_encode :
+    nat -> (('a1*'a2) -> 'a2) -> ('a1 data_t0*'a2) -> 'a2 **)
+
+let fixList_encode size0 encode_A bundle =
+  encode'1 encode_A (fst bundle) (snd bundle)
+
+(** val decode'1 :
+    (('a1*'a2) -> 'a2) -> ('a1*'a2, 'a2) decoder -> nat -> 'a2 -> 'a1
+    list*'a2 **)
+
+let rec decode'1 encode_A decoder_A len b =
+  match len with
+  | O -> [],b
+  | S size' ->
+    let _data,_bin = decode encode_A decoder_A b in
+    let _rest,_bin' = decode'1 encode_A decoder_A size' _bin in
+    (_data::_rest),_bin'
+
+(** val fixList_decode :
+    nat -> (('a1*'a2) -> 'a2) -> ('a1*'a2, 'a2) decoder -> nat -> 'a2 ->
+    'a1 data_t0*'a2 **)
+
+let fixList_decode size0 encode_A decoder_A len b =
+  (fst (decode'1 encode_A decoder_A (min (pred (exp2_nat size0)) len) b)),
+    (snd (decode'1 encode_A decoder_A len b))
+
+(** val fixList_decoder :
+    nat -> n -> (('a1*'a2) -> 'a2) -> ('a1*'a2, 'a2) decoder -> ('a1
+    data_t0*'a2, 'a2) decoder **)
+
+let fixList_decoder size0 len encode_A decoder_A =
+  fixList_decode size0 encode_A decoder_A (N.to_nat len)
+
+type 'a data_t1 = 'a list
+
+(** val encode'2 : (('a1*'a2) -> 'a2) -> 'a1 list -> 'a2 -> 'a2 **)
+
+let rec encode'2 encode_A xs ext =
+  match xs with
+  | [] -> ext
+  | x::xs0 -> encode_A (x,(encode'2 encode_A xs0 ext))
+
+(** val fixList2_encode :
+    nat -> (('a1*'a2) -> 'a2) -> ('a1 data_t1*'a2) -> 'a2 **)
+
+let fixList2_encode size0 encode_A bundle =
+  encode'2 encode_A (fst bundle) (snd bundle)
+
+(** val decode'2 :
+    (('a1*'a2) -> 'a2) -> ('a1*'a2, 'a2) decoder -> nat -> 'a2 -> 'a1
+    list*'a2 **)
+
+let rec decode'2 encode_A decoder_A len b =
+  match len with
+  | O -> [],b
+  | S size' ->
+    let _data,_bin = decode encode_A decoder_A b in
+    let _rest,_bin' = decode'2 encode_A decoder_A size' _bin in
+    (_data::_rest),_bin'
+
+(** val fixList2_decode :
+    nat -> (('a1*'a2) -> 'a2) -> ('a1*'a2, 'a2) decoder -> 'a2 -> 'a1
+    data_t1*'a2 **)
+
+let fixList2_decode size0 encode_A decoder_A b =
+  (fst (decode'2 encode_A decoder_A size0 b)),(snd
+                                                (decode'2 encode_A
+                                                  decoder_A size0 b))
+
+(** val fixList2_decoder :
+    nat -> (('a1*'a2) -> 'a2) -> ('a1*'a2, 'a2) decoder -> ('a1
+    data_t1*'a2, 'a2) decoder **)
+
+let fixList2_decoder size0 encode_A decoder_A =
+  fixList2_decode size0 encode_A decoder_A
+
+(** val zero0 : char **)
+
+let zero0 =
+  '\000'
+
+(** val one0 : char **)
+
+let one0 =
+  '\001'
+
+(** val shift : bool -> char -> char **)
+
+let shift c a =
+  (* If this appears, you're using Ascii internals. Please don't *) (fun f c -> let n = Char.code c in let h i = (n land (1 lsl i)) <> 0 in f (h 0) (h 1) (h 2) (h 3) (h 4) (h 5) (h 6) (h 7))
+    (fun a1 a2 a3 a4 a5 a6 a7 a8 ->
+    (* If this appears, you're using Ascii internals. Please don't *) (fun (b0,b1,b2,b3,b4,b5,b6,b7) -> let f b i = if b then 1 lsl i else 0 in Char.chr (f b0 0 + f b1 1 + f b2 2 + f b3 3 + f b4 4 + f b5 5 + f b6 6 + f b7 7))
+    (c, a1, a2, a3, a4, a5, a6,
+    a7))
+    a
+
+(** val ascii_of_pos : positive -> char **)
+
+let ascii_of_pos =
+  let rec loop n0 p =
+    match n0 with
+    | O -> zero0
+    | S n' ->
+      (match p with
+       | XI p' -> shift true (loop n' p')
+       | XO p' -> shift false (loop n' p')
+       | XH -> one0)
+  in loop (S (S (S (S (S (S (S (S O))))))))
+
+(** val ascii_of_N : n -> char **)
+
+let ascii_of_N = function
+| N0 -> zero0
+| Npos p -> ascii_of_pos p
+
+(** val n_of_digits : bool list -> n **)
+
+let rec n_of_digits = function
+| [] -> N0
+| b::l' ->
+  N.add (if b then Npos XH else N0)
+    (N.mul (Npos (XO XH)) (n_of_digits l'))
+
+(** val n_of_ascii : char -> n **)
+
+let n_of_ascii a =
+  (* If this appears, you're using Ascii internals. Please don't *) (fun f c -> let n = Char.code c in let h i = (n land (1 lsl i)) <> 0 in f (h 0) (h 1) (h 2) (h 3) (h 4) (h 5) (h 6) (h 7))
+    (fun a0 a1 a2 a3 a4 a5 a6 a7 ->
+    n_of_digits (a0::(a1::(a2::(a3::(a4::(a5::(a6::(a7::[])))))))))
+    a
+
+(** val char_encode : char -> bin_t **)
+
+let char_encode c =
+  fixInt_encode (S (S (S (S (S (S (S (S O)))))))) (n_of_ascii c)
+
+(** val char_decode : bin_t -> char*bin_t **)
+
+let char_decode b =
+  let n0,ext = fixInt_decode (S (S (S (S (S (S (S (S O)))))))) b in
+  (ascii_of_N n0),ext
+
+(** val bool_encode : bool -> bin_t **)
+
+let bool_encode b =
+  b::[]
+
+(** val bool_decode : bin_t -> bool*bin_t **)
+
+let bool_decode = function
+| [] -> false,[]
+| x::xs -> x,xs
+
+type word_t = char list
+
+(** val halt : word_t **)
+
+let halt =
+  []
+
+(** val halt_dec : word_t -> bool **)
+
+let halt_dec = function
+| [] -> true
+| a0::l -> false
+
+type name_t = word_t list
+
+(** val encode_word : (word_t*bin_t) -> bool list **)
+
+let encode_word bundle =
+  bin_encode_transform_pair
+    (fixInt_encode (S (S (S (S (S (S (S (S O)))))))))
+    ((fixList_getlength (S (S (S (S (S (S (S (S O)))))))) (fst bundle)),
+    (fixList_encode (S (S (S (S (S (S (S (S O))))))))
+      (bin_encode_transform_pair char_encode) bundle))
+
+(** val word_decoder : (word_t*bin_t, bool list) decoder **)
+
+let word_decoder =
+  decode_unpack (fun data ->
+    fixList_getlength (S (S (S (S (S (S (S (S O)))))))) (fst data))
+    (bin_encode_transform_pair
+      (fixInt_encode (S (S (S (S (S (S (S (S O))))))))))
+    (fixList_encode (S (S (S (S (S (S (S (S O))))))))
+      (bin_encode_transform_pair char_encode))
+    (bin_encode_transform_pair_Decoder
+      (fixInt_encode (S (S (S (S (S (S (S (S O)))))))))
+      (fixInt_decode (S (S (S (S (S (S (S (S O)))))))))) (fun proj ->
+    strengthen_Decoder
+      (fixList_encode (S (S (S (S (S (S (S (S O))))))))
+        (bin_encode_transform_pair char_encode))
+      (fixList_decoder (S (S (S (S (S (S (S (S O)))))))) proj
+        (bin_encode_transform_pair char_encode)
+        (bin_encode_transform_pair_Decoder char_encode char_decode)))
+
+(** val encode_name : (word_t data_t*bin_t) -> bin_t **)
+
+let encode_name =
+  steppingList_encode halt (S (S (S (S (S (S (S (S (S (S (S (S (S (S (S (S
+    (S (S (S (S (S (S (S (S (S (S (S (S (S (S (S (S (S (S (S (S (S (S (S
+    (S (S (S (S (S (S (S (S (S (S (S (S (S (S (S (S (S (S (S (S (S (S (S
+    (S (S (S (S (S (S (S (S (S (S (S (S (S (S (S (S (S (S (S (S (S (S (S
+    (S (S (S (S (S (S (S (S (S (S (S (S (S (S (S (S (S (S (S (S (S (S (S
+    (S (S (S (S (S (S (S (S (S (S (S (S (S (S (S (S (S (S (S (S (S (S (S
+    (S (S (S (S (S (S (S (S (S (S (S (S (S (S (S (S (S (S (S (S (S (S (S
+    (S (S (S (S (S (S (S (S (S (S (S (S (S (S (S (S (S (S (S (S (S (S (S
+    (S (S (S (S (S (S (S (S (S (S (S (S (S (S (S (S (S (S (S (S (S (S (S
+    (S (S (S (S (S (S (S (S (S (S (S (S (S (S (S (S (S (S (S (S (S (S (S
+    (S (S (S (S (S (S (S (S (S (S (S (S (S (S (S (S (S (S (S (S (S (S (S
+    (S (S (S (S (S (S (S (S (S
+    O)))))))))))))))))))))))))))))))))))))))))))))))))))))))))))))))))))))))))))))))))))))))))))))))))))))))))))))))))))))))))))))))))))))))))))))))))))))))))))))))))))))))))))))))))))))))))))))))))))))))))))))))))))))))))))))))))))))))))))))))))))))))))))))))
+    encode_word
+
+(** val name_decoder : (word_t data_t*bin_t, bin_t) decoder **)
+
+let name_decoder =
+  steppingList_decoder halt halt_dec (S (S (S (S (S (S (S (S (S (S (S (S
+    (S (S (S (S (S (S (S (S (S (S (S (S (S (S (S (S (S (S (S (S (S (S (S
+    (S (S (S (S (S (S (S (S (S (S (S (S (S (S (S (S (S (S (S (S (S (S (S
+    (S (S (S (S (S (S (S (S (S (S (S (S (S (S (S (S (S (S (S (S (S (S (S
+    (S (S (S (S (S (S (S (S (S (S (S (S (S (S (S (S (S (S (S (S (S (S (S
+    (S (S (S (S (S (S (S (S (S (S (S (S (S (S (S (S (S (S (S (S (S (S (S
+    (S (S (S (S (S (S (S (S (S (S (S (S (S (S (S (S (S (S (S (S (S (S (S
+    (S (S (S (S (S (S (S (S (S (S (S (S (S (S (S (S (S (S (S (S (S (S (S
+    (S (S (S (S (S (S (S (S (S (S (S (S (S (S (S (S (S (S (S (S (S (S (S
+    (S (S (S (S (S (S (S (S (S (S (S (S (S (S (S (S (S (S (S (S (S (S (S
+    (S (S (S (S (S (S (S (S (S (S (S (S (S (S (S (S (S (S (S (S (S (S (S
+    (S (S (S (S (S (S (S (S (S (S (S (S (S
+    O)))))))))))))))))))))))))))))))))))))))))))))))))))))))))))))))))))))))))))))))))))))))))))))))))))))))))))))))))))))))))))))))))))))))))))))))))))))))))))))))))))))))))))))))))))))))))))))))))))))))))))))))))))))))))))))))))))))))))))))))))))))))))))))))
+    encode_word word_decoder
+
+type type_t =
+| A
+| CNAME
+| NS
+| MX
+
+type class_t =
+| IN
+| CH
+| HS
+
+(** val fixInt_of_type : type_t -> n **)
+
+let fixInt_of_type = function
+| A -> Npos XH
+| CNAME -> Npos (XI (XO XH))
+| NS -> Npos (XO XH)
+| MX -> Npos (XI (XI (XI XH)))
+
+(** val fixInt_of_class : class_t -> n **)
+
+let fixInt_of_class = function
+| IN -> Npos XH
+| CH -> Npos (XI XH)
+| HS -> Npos (XO (XO XH))
+
+(** val type_to_FixInt_decoder : (type_t, n) decoder **)
+
+let type_to_FixInt_decoder n0 =
+  if N.eq_dec n0 (Npos XH)
+  then A
+  else if N.eq_dec n0 (Npos (XI (XO XH)))
+       then CNAME
+       else if N.eq_dec n0 (Npos (XO XH)) then NS else MX
+
+(** val class_to_FixInt_decoder : (class_t, n) decoder **)
+
+let class_to_FixInt_decoder n0 =
+  if N.eq_dec n0 (Npos XH)
+  then IN
+  else if N.eq_dec n0 (Npos (XI XH)) then CH else HS
+
+type question_t = { qname : name_t; qtype : type_t; qclass : class_t }
+
+(** val qname : question_t -> name_t **)
+
+let qname x = x.qname
+
+(** val qtype : question_t -> type_t **)
+
+let qtype x = x.qtype
+
+(** val qclass : question_t -> class_t **)
+
+let qclass x = x.qclass
+
+(** val encode_question : (question_t*bin_t) -> bin_t **)
+
+let encode_question bundle =
+  encode_name
+    ((fst bundle).qname,(bin_encode_transform_pair
+                          (fixInt_encode (S (S (S (S (S (S (S (S (S (S (S
+                            (S (S (S (S (S O)))))))))))))))))
+                          ((fixInt_of_type (fst bundle).qtype),(bin_encode_transform_pair
+                                                                 (fixInt_encode
+                                                                 (S (S (S
+                                                                 (S (S (S
+                                                                 (S (S (S
+                                                                 (S (S (S
+                                                                 (S (S (S
+                                                                 (S
+                                                                 O)))))))))))))))))
+                                                                 (
+                                                                 (fixInt_of_class
+                                                                 (fst
+                                                                 bundle).qclass),
+                                                                 (snd
+                                                                 bundle))))))
+
+(** val question_decoder : (question_t*bin_t, bin_t) decoder **)
+
+let question_decoder =
+  decode_unpack (fun data -> (fst data).qname) encode_name (fun data ->
+    bin_encode_transform_pair
+      (fixInt_encode (S (S (S (S (S (S (S (S (S (S (S (S (S (S (S (S
+        O)))))))))))))))))
+      ((fixInt_of_type (fst data).qtype),(bin_encode_transform_pair
+                                           (fixInt_encode (S (S (S (S (S
+                                             (S (S (S (S (S (S (S (S (S (S
+                                             (S O)))))))))))))))))
+                                           ((fixInt_of_class
+                                              (fst data).qclass),(snd
+                                                                 data)))))
+    name_decoder (fun proj ->
+    decode_unpack (fun data -> (fst data).qtype) (fun bundle ->
+      bin_encode_transform_pair
+        (fixInt_encode (S (S (S (S (S (S (S (S (S (S (S (S (S (S (S (S
+          O))))))))))))))))) ((fixInt_of_type (fst bundle)),(snd bundle)))
+      (fun data ->
+      bin_encode_transform_pair
+        (fixInt_encode (S (S (S (S (S (S (S (S (S (S (S (S (S (S (S (S
+          O)))))))))))))))))
+        ((fixInt_of_class (fst data).qclass),(snd data)))
+      (nested_decoder (fun data -> (fixInt_of_type (fst data)),(snd data))
+        (bin_encode_transform_pair
+          (fixInt_encode (S (S (S (S (S (S (S (S (S (S (S (S (S (S (S (S
+            O))))))))))))))))))
+        (unprod_decoder fixInt_of_type type_to_FixInt_decoder)
+        (bin_encode_transform_pair_Decoder
+          (fixInt_encode (S (S (S (S (S (S (S (S (S (S (S (S (S (S (S (S
+            O)))))))))))))))))
+          (fixInt_decode (S (S (S (S (S (S (S (S (S (S (S (S (S (S (S (S
+            O))))))))))))))))))) (fun proj0 ->
+      decode_unpack (fun data -> (fst data).qclass) (fun bundle ->
+        bin_encode_transform_pair
+          (fixInt_encode (S (S (S (S (S (S (S (S (S (S (S (S (S (S (S (S
+            O)))))))))))))))))
+          ((fixInt_of_class (fst bundle)),(snd bundle))) (fun data ->
+        let x,y = data in y)
+        (nested_decoder (fun data ->
+          (fixInt_of_class (fst data)),(snd data))
+          (bin_encode_transform_pair
+            (fixInt_encode (S (S (S (S (S (S (S (S (S (S (S (S (S (S (S (S
+              O))))))))))))))))))
+          (unprod_decoder fixInt_of_class class_to_FixInt_decoder)
+          (bin_encode_transform_pair_Decoder
+            (fixInt_encode (S (S (S (S (S (S (S (S (S (S (S (S (S (S (S (S
+              O)))))))))))))))))
+            (fixInt_decode (S (S (S (S (S (S (S (S (S (S (S (S (S (S (S (S
+              O))))))))))))))))))) (fun proj1 b -> { qname = proj; qtype =
+        proj0; qclass = proj1 },b)))
+
+type packet_t = { pid : bool list; pmask : bool list;
+                  pquestion : question_t list; panswer : question_t list;
+                  pauthority : question_t list;
+                  padditional : question_t list }
+
+(** val pid : packet_t -> bool list **)
+
+let pid x = x.pid
+
+(** val pmask : packet_t -> bool list **)
+
+let pmask x = x.pmask
+
+(** val pquestion : packet_t -> question_t list **)
+
+let pquestion x = x.pquestion
+
+(** val panswer : packet_t -> question_t list **)
+
+let panswer x = x.panswer
+
+(** val pauthority : packet_t -> question_t list **)
+
+let pauthority x = x.pauthority
+
+(** val padditional : packet_t -> question_t list **)
+
+let padditional x = x.padditional
+
+(** val packet_decoder : (packet_t*bin_t, bin_t) decoder **)
+
+let packet_decoder =
+  decode_unpack (fun data -> (fst data).pid)
+    (fixList2_encode (S (S (S (S (S (S (S (S (S (S (S (S (S (S (S (S
+      O)))))))))))))))) (bin_encode_transform_pair bool_encode))
+    (fun data ->
+    fixList2_encode (S (S (S (S (S (S (S (S (S (S (S (S (S (S (S (S
+      O)))))))))))))))) (bin_encode_transform_pair bool_encode)
+      ((fst data).pmask,(bin_encode_transform_pair
+                          (fixInt_encode (S (S (S (S (S (S (S (S (S (S (S
+                            (S (S (S (S (S O)))))))))))))))))
+                          ((fixList_getlength (S (S (S (S (S (S (S (S (S
+                             (S (S (S (S (S (S (S O))))))))))))))))
+                             (fst data).pquestion),(bin_encode_transform_pair
+                                                     (fixInt_encode (S (S
+                                                       (S (S (S (S (S (S
+                                                       (S (S (S (S (S (S
+                                                       (S (S
+                                                       O)))))))))))))))))
+                                                     ((fixList_getlength
+                                                        (S (S (S (S (S (S
+                                                        (S (S (S (S (S (S
+                                                        (S (S (S (S
+                                                        O))))))))))))))))
+                                                        (fst data).panswer),
+                                                     (bin_encode_transform_pair
+                                                       (fixInt_encode (S
+                                                         (S (S (S (S (S (S
+                                                         (S (S (S (S (S (S
+                                                         (S (S (S
+                                                         O)))))))))))))))))
+                                                       ((fixList_getlength
+                                                          (S (S (S (S (S
+                                                          (S (S (S (S (S
+                                                          (S (S (S (S (S
+                                                          (S
+                                                          O))))))))))))))))
+                                                          (fst data).pauthority),
+                                                       (bin_encode_transform_pair
+                                                         (fixInt_encode (S
+                                                           (S (S (S (S (S
+                                                           (S (S (S (S (S
+                                                           (S (S (S (S (S
+                                                           O)))))))))))))))))
+                                                         ((fixList_getlength
+                                                            (S (S (S (S (S
+                                                            (S (S (S (S (S
+                                                            (S (S (S (S (S
+                                                            (S
+                                                            O))))))))))))))))
+                                                            (fst data).padditional),
+                                                         (fixList_encode
+                                                           (S (S (S (S (S
+                                                           (S (S (S (S (S
+                                                           (S (S (S (S (S
+                                                           (S
+                                                           O))))))))))))))))
+                                                           encode_question
+                                                           ((fst data).pquestion,
+                                                           (fixList_encode
+                                                             (S (S (S (S
+                                                             (S (S (S (S
+                                                             (S (S (S (S
+                                                             (S (S (S (S
+                                                             O))))))))))))))))
+                                                             encode_question
+                                                             ((fst data).panswer,
+                                                             (fixList_encode
+                                                               (S (S (S (S
+                                                               (S (S (S (S
+                                                               (S (S (S (S
+                                                               (S (S (S (S
+                                                               O))))))))))))))))
+                                                               encode_question
+                                                               ((fst data).pauthority,
+                                                               (fixList_encode
+                                                                 (S (S (S
+                                                                 (S (S (S
+                                                                 (S (S (S
+                                                                 (S (S (S
+                                                                 (S (S (S
+                                                                 (S
+                                                                 O))))))))))))))))
+                                                                 encode_question
+                                                                 (
+                                                                 (fst
+                                                                 data).padditional,
+                                                                 (snd
+                                                                 data)))))))))))))))))))
+    (fixList2_decoder (S (S (S (S (S (S (S (S (S (S (S (S (S (S (S (S
+      O)))))))))))))))) (bin_encode_transform_pair bool_encode)
+      (bin_encode_transform_pair_Decoder bool_encode bool_decode))
+    (fun proj ->
+    decode_unpack (fun data -> (fst data).pmask)
+      (fixList2_encode (S (S (S (S (S (S (S (S (S (S (S (S (S (S (S (S
+        O)))))))))))))))) (bin_encode_transform_pair bool_encode))
+      (fun data ->
+      bin_encode_transform_pair
+        (fixInt_encode (S (S (S (S (S (S (S (S (S (S (S (S (S (S (S (S
+          O)))))))))))))))))
+        ((fixList_getlength (S (S (S (S (S (S (S (S (S (S (S (S (S (S (S
+           (S O)))))))))))))))) (fst data).pquestion),(bin_encode_transform_pair
+                                                        (fixInt_encode (S
+                                                          (S (S (S (S (S
+                                                          (S (S (S (S (S
+                                                          (S (S (S (S (S
+                                                          O)))))))))))))))))
+                                                        ((fixList_getlength
+                                                           (S (S (S (S (S
+                                                           (S (S (S (S (S
+                                                           (S (S (S (S (S
+                                                           (S
+                                                           O))))))))))))))))
+                                                           (fst data).panswer),
+                                                        (bin_encode_transform_pair
+                                                          (fixInt_encode
+                                                            (S (S (S (S (S
+                                                            (S (S (S (S (S
+                                                            (S (S (S (S (S
+                                                            (S
+                                                            O)))))))))))))))))
+                                                          ((fixList_getlength
+                                                             (S (S (S (S
+                                                             (S (S (S (S
+                                                             (S (S (S (S
+                                                             (S (S (S (S
+                                                             O))))))))))))))))
+                                                             (fst data).pauthority),
+                                                          (bin_encode_transform_pair
+                                                            (fixInt_encode
+                                                              (S (S (S (S
+                                                              (S (S (S (S
+                                                              (S (S (S (S
+                                                              (S (S (S (S
+                                                              O)))))))))))))))))
+                                                            ((fixList_getlength
+                                                               (S (S (S (S
+                                                               (S (S (S (S
+                                                               (S (S (S (S
+                                                               (S (S (S (S
+                                                               O))))))))))))))))
+                                                               (fst data).padditional),
+                                                            (fixList_encode
+                                                              (S (S (S (S
+                                                              (S (S (S (S
+                                                              (S (S (S (S
+                                                              (S (S (S (S
+                                                              O))))))))))))))))
+                                                              encode_question
+                                                              ((fst data).pquestion,
+                                                              (fixList_encode
+                                                                (S (S (S
+                                                                (S (S (S
+                                                                (S (S (S
+                                                                (S (S (S
+                                                                (S (S (S
+                                                                (S
+                                                                O))))))))))))))))
+                                                                encode_question
+                                                                ((fst
+                                                                 data).panswer,
+                                                                (fixList_encode
+                                                                 (S (S (S
+                                                                 (S (S (S
+                                                                 (S (S (S
+                                                                 (S (S (S
+                                                                 (S (S (S
+                                                                 (S
+                                                                 O))))))))))))))))
+                                                                 encode_question
+                                                                 ((fst
+                                                                 data).pauthority,
+                                                                 (fixList_encode
+                                                                 (S (S (S
+                                                                 (S (S (S
+                                                                 (S (S (S
+                                                                 (S (S (S
+                                                                 (S (S (S
+                                                                 (S
+                                                                 O))))))))))))))))
+                                                                 encode_question
+                                                                 ((fst
+                                                                 data).padditional,
+                                                                 (snd
+                                                                 data)))))))))))))))))
+      (fixList2_decoder (S (S (S (S (S (S (S (S (S (S (S (S (S (S (S (S
+        O)))))))))))))))) (bin_encode_transform_pair bool_encode)
+        (bin_encode_transform_pair_Decoder bool_encode bool_decode))
+      (fun proj0 ->
+      decode_unpack (fun data ->
+        fixList_getlength (S (S (S (S (S (S (S (S (S (S (S (S (S (S (S (S
+          O)))))))))))))))) (fst data).pquestion)
+        (bin_encode_transform_pair
+          (fixInt_encode (S (S (S (S (S (S (S (S (S (S (S (S (S (S (S (S
+            O)))))))))))))))))) (fun data ->
+        bin_encode_transform_pair
+          (fixInt_encode (S (S (S (S (S (S (S (S (S (S (S (S (S (S (S (S
+            O)))))))))))))))))
+          ((fixList_getlength (S (S (S (S (S (S (S (S (S (S (S (S (S (S (S
+             (S O)))))))))))))))) (fst data).panswer),(bin_encode_transform_pair
+                                                        (fixInt_encode (S
+                                                          (S (S (S (S (S
+                                                          (S (S (S (S (S
+                                                          (S (S (S (S (S
+                                                          O)))))))))))))))))
+                                                        ((fixList_getlength
+                                                           (S (S (S (S (S
+                                                           (S (S (S (S (S
+                                                           (S (S (S (S (S
+                                                           (S
+                                                           O))))))))))))))))
+                                                           (fst data).pauthority),
+                                                        (bin_encode_transform_pair
+                                                          (fixInt_encode
+                                                            (S (S (S (S (S
+                                                            (S (S (S (S (S
+                                                            (S (S (S (S (S
+                                                            (S
+                                                            O)))))))))))))))))
+                                                          ((fixList_getlength
+                                                             (S (S (S (S
+                                                             (S (S (S (S
+                                                             (S (S (S (S
+                                                             (S (S (S (S
+                                                             O))))))))))))))))
+                                                             (fst data).padditional),
+                                                          (fixList_encode
+                                                            (S (S (S (S (S
+                                                            (S (S (S (S (S
+                                                            (S (S (S (S (S
+                                                            (S
+                                                            O))))))))))))))))
+                                                            encode_question
+                                                            ((fst data).pquestion,
+                                                            (fixList_encode
+                                                              (S (S (S (S
+                                                              (S (S (S (S
+                                                              (S (S (S (S
+                                                              (S (S (S (S
+                                                              O))))))))))))))))
+                                                              encode_question
+                                                              ((fst data).panswer,
+                                                              (fixList_encode
+                                                                (S (S (S
+                                                                (S (S (S
+                                                                (S (S (S
+                                                                (S (S (S
+                                                                (S (S (S
+                                                                (S
+                                                                O))))))))))))))))
+                                                                encode_question
+                                                                ((fst
+                                                                 data).pauthority,
+                                                                (fixList_encode
+                                                                 (S (S (S
+                                                                 (S (S (S
+                                                                 (S (S (S
+                                                                 (S (S (S
+                                                                 (S (S (S
+                                                                 (S
+                                                                 O))))))))))))))))
+                                                                 encode_question
+                                                                 ((fst
+                                                                 data).padditional,
+                                                                 (snd
+                                                                 data)))))))))))))))
+        (bin_encode_transform_pair_Decoder
+          (fixInt_encode (S (S (S (S (S (S (S (S (S (S (S (S (S (S (S (S
+            O)))))))))))))))))
+          (fixInt_decode (S (S (S (S (S (S (S (S (S (S (S (S (S (S (S (S
+            O)))))))))))))))))) (fun proj1 ->
+        decode_unpack (fun data ->
+          fixList_getlength (S (S (S (S (S (S (S (S (S (S (S (S (S (S (S
+            (S O)))))))))))))))) (fst data).panswer)
+          (bin_encode_transform_pair
+            (fixInt_encode (S (S (S (S (S (S (S (S (S (S (S (S (S (S (S (S
+              O)))))))))))))))))) (fun data ->
+          bin_encode_transform_pair
+            (fixInt_encode (S (S (S (S (S (S (S (S (S (S (S (S (S (S (S (S
+              O)))))))))))))))))
+            ((fixList_getlength (S (S (S (S (S (S (S (S (S (S (S (S (S (S
+               (S (S O)))))))))))))))) (fst data).pauthority),(bin_encode_transform_pair
+                                                                (fixInt_encode
+                                                                 (S (S (S
+                                                                 (S (S (S
+                                                                 (S (S (S
+                                                                 (S (S (S
+                                                                 (S (S (S
+                                                                 (S
+                                                                 O)))))))))))))))))
+                                                                ((fixList_getlength
+                                                                 (S (S (S
+                                                                 (S (S (S
+                                                                 (S (S (S
+                                                                 (S (S (S
+                                                                 (S (S (S
+                                                                 (S
+                                                                 O))))))))))))))))
+                                                                 (fst
+                                                                 data).padditional),
+                                                                (fixList_encode
+                                                                 (S (S (S
+                                                                 (S (S (S
+                                                                 (S (S (S
+                                                                 (S (S (S
+                                                                 (S (S (S
+                                                                 (S
+                                                                 O))))))))))))))))
+                                                                 encode_question
+                                                                 ((fst
+                                                                 data).pquestion,
+                                                                 (fixList_encode
+                                                                 (S (S (S
+                                                                 (S (S (S
+                                                                 (S (S (S
+                                                                 (S (S (S
+                                                                 (S (S (S
+                                                                 (S
+                                                                 O))))))))))))))))
+                                                                 encode_question
+                                                                 ((fst
+                                                                 data).panswer,
+                                                                 (fixList_encode
+                                                                 (S (S (S
+                                                                 (S (S (S
+                                                                 (S (S (S
+                                                                 (S (S (S
+                                                                 (S (S (S
+                                                                 (S
+                                                                 O))))))))))))))))
+                                                                 encode_question
+                                                                 ((fst
+                                                                 data).pauthority,
+                                                                 (fixList_encode
+                                                                 (S (S (S
+                                                                 (S (S (S
+                                                                 (S (S (S
+                                                                 (S (S (S
+                                                                 (S (S (S
+                                                                 (S
+                                                                 O))))))))))))))))
+                                                                 encode_question
+                                                                 ((fst
+                                                                 data).padditional,
+                                                                 (snd
+                                                                 data)))))))))))))
+          (bin_encode_transform_pair_Decoder
+            (fixInt_encode (S (S (S (S (S (S (S (S (S (S (S (S (S (S (S (S
+              O)))))))))))))))))
+            (fixInt_decode (S (S (S (S (S (S (S (S (S (S (S (S (S (S (S (S
+              O)))))))))))))))))) (fun proj2 ->
+          decode_unpack (fun data ->
+            fixList_getlength (S (S (S (S (S (S (S (S (S (S (S (S (S (S (S
+              (S O)))))))))))))))) (fst data).pauthority)
+            (bin_encode_transform_pair
+              (fixInt_encode (S (S (S (S (S (S (S (S (S (S (S (S (S (S (S
+                (S O)))))))))))))))))) (fun data ->
+            bin_encode_transform_pair
+              (fixInt_encode (S (S (S (S (S (S (S (S (S (S (S (S (S (S (S
+                (S O)))))))))))))))))
+              ((fixList_getlength (S (S (S (S (S (S (S (S (S (S (S (S (S
+                 (S (S (S O)))))))))))))))) (fst data).padditional),
+              (fixList_encode (S (S (S (S (S (S (S (S (S (S (S (S (S (S (S
+                (S O)))))))))))))))) encode_question
+                ((fst data).pquestion,(fixList_encode (S (S (S (S (S (S (S
+                                        (S (S (S (S (S (S (S (S (S
+                                        O)))))))))))))))) encode_question
+                                        ((fst data).panswer,(fixList_encode
+                                                              (S (S (S (S
+                                                              (S (S (S (S
+                                                              (S (S (S (S
+                                                              (S (S (S (S
+                                                              O))))))))))))))))
+                                                              encode_question
+                                                              ((fst data).pauthority,
+                                                              (fixList_encode
+                                                                (S (S (S
+                                                                (S (S (S
+                                                                (S (S (S
+                                                                (S (S (S
+                                                                (S (S (S
+                                                                (S
+                                                                O))))))))))))))))
+                                                                encode_question
+                                                                ((fst
+                                                                 data).padditional,
+                                                                (snd data)))))))))))
+            (bin_encode_transform_pair_Decoder
+              (fixInt_encode (S (S (S (S (S (S (S (S (S (S (S (S (S (S (S
+                (S O)))))))))))))))))
+              (fixInt_decode (S (S (S (S (S (S (S (S (S (S (S (S (S (S (S
+                (S O)))))))))))))))))) (fun proj3 ->
+            decode_unpack (fun data ->
+              fixList_getlength (S (S (S (S (S (S (S (S (S (S (S (S (S (S
+                (S (S O)))))))))))))))) (fst data).padditional)
+              (bin_encode_transform_pair
+                (fixInt_encode (S (S (S (S (S (S (S (S (S (S (S (S (S (S
+                  (S (S O)))))))))))))))))) (fun data ->
+              fixList_encode (S (S (S (S (S (S (S (S (S (S (S (S (S (S (S
+                (S O)))))))))))))))) encode_question
+                ((fst data).pquestion,(fixList_encode (S (S (S (S (S (S (S
+                                        (S (S (S (S (S (S (S (S (S
+                                        O)))))))))))))))) encode_question
+                                        ((fst data).panswer,(fixList_encode
+                                                              (S (S (S (S
+                                                              (S (S (S (S
+                                                              (S (S (S (S
+                                                              (S (S (S (S
+                                                              O))))))))))))))))
+                                                              encode_question
+                                                              ((fst data).pauthority,
+                                                              (fixList_encode
+                                                                (S (S (S
+                                                                (S (S (S
+                                                                (S (S (S
+                                                                (S (S (S
+                                                                (S (S (S
+                                                                (S
+                                                                O))))))))))))))))
+                                                                encode_question
+                                                                ((fst
+                                                                 data).padditional,
+                                                                (snd data)))))))))
+              (bin_encode_transform_pair_Decoder
+                (fixInt_encode (S (S (S (S (S (S (S (S (S (S (S (S (S (S
+                  (S (S O)))))))))))))))))
+                (fixInt_decode (S (S (S (S (S (S (S (S (S (S (S (S (S (S
+                  (S (S O)))))))))))))))))) (fun proj4 ->
+              decode_unpack (fun data -> (fst data).pquestion)
+                (fixList_encode (S (S (S (S (S (S (S (S (S (S (S (S (S (S
+                  (S (S O)))))))))))))))) encode_question) (fun data ->
+                fixList_encode (S (S (S (S (S (S (S (S (S (S (S (S (S (S
+                  (S (S O)))))))))))))))) encode_question
+                  ((fst data).panswer,(fixList_encode (S (S (S (S (S (S (S
+                                        (S (S (S (S (S (S (S (S (S
+                                        O)))))))))))))))) encode_question
+                                        ((fst data).pauthority,(fixList_encode
+                                                                 (S (S (S
+                                                                 (S (S (S
+                                                                 (S (S (S
+                                                                 (S (S (S
+                                                                 (S (S (S
+                                                                 (S
+                                                                 O))))))))))))))))
+                                                                 encode_question
+                                                                 (
+                                                                 (fst
+                                                                 data).padditional,
+                                                                 (snd
+                                                                 data)))))))
+                (fixList_decoder (S (S (S (S (S (S (S (S (S (S (S (S (S (S
+                  (S (S O)))))))))))))))) proj1 encode_question
+                  question_decoder) (fun proj5 ->
+                decode_unpack (fun data -> (fst data).panswer)
+                  (fixList_encode (S (S (S (S (S (S (S (S (S (S (S (S (S
+                    (S (S (S O)))))))))))))))) encode_question)
+                  (fun data ->
+                  fixList_encode (S (S (S (S (S (S (S (S (S (S (S (S (S (S
+                    (S (S O)))))))))))))))) encode_question
+                    ((fst data).pauthority,(fixList_encode (S (S (S (S (S
+                                             (S (S (S (S (S (S (S (S (S (S
+                                             (S O))))))))))))))))
+                                             encode_question
+                                             ((fst data).padditional,
+                                             (snd data)))))
+                  (fixList_decoder (S (S (S (S (S (S (S (S (S (S (S (S (S
+                    (S (S (S O)))))))))))))))) proj2 encode_question
+                    question_decoder) (fun proj6 ->
+                  decode_unpack (fun data -> (fst data).pauthority)
+                    (fixList_encode (S (S (S (S (S (S (S (S (S (S (S (S (S
+                      (S (S (S O)))))))))))))))) encode_question)
+                    (fun data ->
+                    fixList_encode (S (S (S (S (S (S (S (S (S (S (S (S (S
+                      (S (S (S O)))))))))))))))) encode_question
+                      ((fst data).padditional,(snd data)))
+                    (fixList_decoder (S (S (S (S (S (S (S (S (S (S (S (S
+                      (S (S (S (S O)))))))))))))))) proj3 encode_question
+                      question_decoder) (fun proj7 ->
+                    decode_unpack (fun data -> (fst data).padditional)
+                      (fixList_encode (S (S (S (S (S (S (S (S (S (S (S (S
+                        (S (S (S (S O)))))))))))))))) encode_question) snd
+                      (fixList_decoder (S (S (S (S (S (S (S (S (S (S (S (S
+                        (S (S (S (S O)))))))))))))))) proj4
+                        encode_question question_decoder) (fun proj8 b ->
+                      { pid = proj; pmask = proj0; pquestion = proj5;
+                      panswer = proj6; pauthority = proj7; padditional =
+                      proj8 },b))))))))))
+
+let packet_bin = [true; true; false; true; true; false; true; true; false; true;
+  false; false; false; false; true; false; false; false; false; false;
+  false; false; false; true; false; false; false; false; false; false;
+  false; false; false; false; false; false; false; false; false; false;
+  false; false; false; false; false; false; false; true; false; false;
+  false; false; false; false; false; false; false; false; false; false;
+  false; false; false; false; false; false; false; false; false; false;
+  false; false; false; false; false; false; false; false; false; false;
+  false; false; false; false; false; false; false; false; false; false;
+  false; false; false; false; false; false; false; false; false; false;
+  false; false; true; true; false; true; true; true; false; true;
+  true; true; false; true; true; true; false; true; true; true;
+  false; true; true; true; false; true; true; true; false; false;
+  false; false; true; true; false; false; false; true; true; false;
+  true; true; true; false; false; true; true; false; true; true;
+  true; true; false; true; true; true; false; false; true; false;
+  false; true; true; true; false; true; false; false; false; true;
+  true; false; true; false; false; false; false; true; true; false;
+  false; true; false; true; false; true; true; false; false; false;
+  false; true; false; true; true; true; false; false; true; true;
+  false; true; true; true; false; true; false; false; false; true;
+  true; false; false; true; false; true; false; true; true; true;
+  false; false; true; false; false; true; true; false; true; true;
+  true; false; false; false; false; false; false; false; true; true;
+  false; true; true; false; false; true; false; true; false; true;
+  true; false; false; true; false; false; false; true; true; true;
+  false; true; false; true; false; false; false; false; false; false;
+  false; false; false; false; false; false; false; false; false; false;
+  false; false; false; false; false; false; false; true; false; false;
+  false; false; false; false; false; false; false; false; false; false;
+  false; false; false; true; ];;
+
+let answer = packet_decoder packet_bin;;
