src/BinEncoders/Examples/Dns.v
@@ -1,130 +1,245 @@
-Require Import Coq.Strings.String
-               Coq.Bool.Bvector.
 Require Import Fiat.BinEncoders.Specs
-               Fiat.BinEncoders.Libraries.Core
+               Fiat.BinEncoders.Libraries.Helpers
+               Fiat.BinEncoders.Libraries.Sig
+               Fiat.BinEncoders.Libraries.BinCore
                Fiat.BinEncoders.Libraries.FixInt
+               Fiat.BinEncoders.Libraries.SteppingList
+               Fiat.BinEncoders.Libraries.FixList
+               Fiat.BinEncoders.Libraries.FixList2
                Fiat.BinEncoders.Libraries.Char
-               Fiat.BinEncoders.Libraries.VList.
+               Fiat.BinEncoders.Libraries.Bool
+               Coq.Strings.Ascii.
 
 Set Implicit Arguments.
 
-Section DnsPacket.
+Definition word_t := { s : list ascii | length s < exp2_nat 8 }.
 
-  Inductive RRecordType := A | CNAME | NS | MX.
-  Inductive RRecordClass := IN | CH | HS.
+Definition halt : word_t.
+  refine (exist _ nil _).
+  rewrite Compare_dec.nat_compare_lt; eauto.
+Defined.
 
-  (* find a way to do this systematically *)
-  Definition RRecordTypeToFixInt (t : RRecordType) : {n | (n < exp2 16)%N}.
-    refine (match t with
-            | A     => exist _ (1%N) _
-            | CNAME => exist _ (5%N) _
-            | NS    => exist _ (2%N) _
-            | MX    => exist _ (15%N) _
-            end); rewrite <- N.compare_lt_iff; eauto.
-  Defined.
+Definition halt_dec (a : word_t) : {a = halt} + {a <> halt}.
+  unfold halt; destruct a as [word word_pf].
+  destruct word eqn: eq; subst.
+  - left. subst. eapply sig_equivalence. eauto.
+  - right. intro. inversion H.
+Defined.
 
-  Definition RRecordClassToFixInt (c : RRecordClass) : {n | (n < exp2 16)%N}.
-    refine (match c with
-            | IN => exist _ (1%N) _
-            | CH => exist _ (3%N) _
-            | HS => exist _ (4%N) _
-            end); rewrite <- N.compare_lt_iff; eauto.
-  Defined.
+Definition name_t := { s : list word_t | length s <= 255 /\ forall x, In x s -> x <> halt }.
 
-  Global Instance RRType_decoder
-    : decoder (fun _ => True) RRecordTypeToFixInt :=
-    { decode := fun n => if N.eq_dec (proj1_sig n) (1%N) then A
-                         else if N.eq_dec (proj1_sig n) (5%N) then CNAME
-                         else if N.eq_dec (proj1_sig n) (2%N) then NS
-                         else MX;
-      decode_correct := _ }.
-  Proof.
-    intros data _; destruct data; eauto.
-  Defined.
+Definition encode_word (bundle : word_t * bin_t) :=
+  bin_encode_transform_pair (@FixInt_encode _) (FixList_getlength (fst bundle),
+    FixList_encode (bin_encode_transform_pair Char_encode) bundle).
 
-  Global Instance RRClass_decoder
-    : decoder (fun _ => True) RRecordClassToFixInt :=
-    { decode := fun n => if N.eq_dec (proj1_sig n) (1%N) then IN
-                         else if N.eq_dec (proj1_sig n) (3%N) then CH
-                         else HS;
-      decode_correct := _ }.
-  Proof.
-    intros data _; destruct data; eauto.
-  Defined.
+Global Instance word_decoder
+  : decoder (fun _ => True) encode_word.
+Proof.
+  unfold encode_word.
+  eapply decode_unpack.
+  instantiate (1:=fun _ => True). intuition. cbv beta.
+  eapply bin_encode_transform_pair_Decoder. eapply FixInt_encode_correct.
+  intro proj.
+  eapply strengthen_Decoder.
+  eapply FixList_decoder with (size:=8) (len:=proj).
+  instantiate (1:=fun _ => True). intuition. cbv beta.
+  eapply bin_encode_transform_pair_Decoder. eapply Char_encode_correct.
+  firstorder.
+Defined.
 
+Definition encode_name := @SteppingList_encode _ _ halt 255 encode_word.
 
-  Record question :=
-    { qname : list (list ascii);
-      qtype : RRecordType;
-      qclass : RRecordClass }.
+Global Instance name_decoder
+  : decoder (SteppingList_predicate (fun _ => True)) encode_name.
+Proof.
+  eapply SteppingList_decoder.
+  eapply halt_dec.
+  eapply word_decoder.
+Defined.
 
-  Global Instance App_decoder
-         (A : Type)
-         (encode_A : A -> bin)
-         (A_Decoder : decoder (fun _ => True) encode_A)
-    : decoder (fun _ => True)
-              (fun _bundle : A * bin => let (_data, _bin) := _bundle in encode_A _data ++ _bin).
-  Admitted.
+Inductive type_t := A | CNAME | NS | MX.
+Inductive class_t := IN | CH | HS.
 
-  Definition question_encode (q : question) :=
-    VList_encode (VList_encode_pair Char_encode_pair) (qname q) ++
-    FixInt_encode _ (RRecordTypeToFixInt (qtype q)) ++
-    FixInt_encode _ (RRecordClassToFixInt (qclass q)).
+Definition FixInt_of_type (t : type_t) : {n | (n < exp2 16)%N}.
+  refine (match t with
+          | A     => exist _ (1%N) _
+          | CNAME => exist _ (5%N) _
+          | NS    => exist _ (2%N) _
+          | MX    => exist _ (15%N) _
+          end); rewrite <- N.compare_lt_iff; eauto.
+Defined.
 
-  Definition question_decode :
-    { question_decode | question_encode <+> question_decode }.
-  Proof.
-    unfold question_encode.
-    eexists.
+Definition FixInt_of_class (c : class_t) : {n | (n < exp2 16)%N}.
+  refine (match c with
+          | IN => exist _ (1%N) _
+          | CH => exist _ (3%N) _
+          | HS => exist _ (4%N) _
+          end); rewrite <- N.compare_lt_iff; eauto.
+Defined.
 
-    match goal with
-    | |- encode_decode_correct _ (fun data => ?e1 (_ data) ++ @?e2 data) _ =>
-        eapply decode_unpack with
-           (encode1:=fun (_bundle : _ * bin) =>
-                       let (_proj, _bin) := _bundle
-                       in  e1 _proj ++ _bin)
-    end.
-    instantiate (1:=fun _ => True). intuition. cbv beta. eapply decode_correct. intro.
+Global Instance type_to_FixInt_decoder
+  : decoder (fun _ => True) FixInt_of_type :=
+  { decode := fun n => if N.eq_dec (proj1_sig n) (1%N) then A
+                       else if N.eq_dec (proj1_sig n) (5%N) then CNAME
+                       else if N.eq_dec (proj1_sig n) (2%N) then NS
+                       else MX }.
+Proof.
+  intros data _; destruct data; eauto.
+Defined.
 
-    match goal with
-    | |- encode_decode_correct _ (fun data => ?e1 (?p1 (_ data)) ++ @?e2 data) _ =>
-        eapply decode_unpack with
-           (encode1:=fun (_bundle : _ * bin) =>
-                       let (_proj, _bin) := _bundle
-                       in  e1 (p1 _proj) ++ _bin)
-    end.
-    instantiate (1:=fun _ => True). intuition. cbv beta. eapply decode_correct. intro.
+Global Instance class_to_FixInt_decoder
+  : decoder (fun _ => True) FixInt_of_class :=
+  { decode := fun n => if N.eq_dec (proj1_sig n) (1%N) then IN
+                       else if N.eq_dec (proj1_sig n) (3%N) then CH
+                       else HS }.
+Proof.
+  intros data _; destruct data; eauto.
+Defined.
 
-    (* final step! *)
-    eapply decode_moveproj with
-      (encode:=fun c => FixInt_encode 16 (RRecordClassToFixInt c))
-      (constr:=fun _ => Build_question _ _ _).
-    instantiate (1:=fun _ => True). intuition. cbv beta. eapply decode_correct. intro.
-    intros. destruct data.
-    intuition. simpl in *. subst. reflexivity.
+Record question_t :=
+  { qname : name_t;
+    qtype : type_t;
+    qclass : class_t }.
 
-    (*
-    match goal with
-    | |- encode_decode_correct _ (fun data => ?e1 (?p1 (_ data)) ++ @?e2 data) _ =>
-        eapply decode_unpack with
-           (encode1:=fun (_bundle : _ * bin) =>
-                       let (_proj, _bin) := _bundle
-                       in  e1 (p1 _proj) ++ _bin)
-    end.
-    instantiate (1:=fun _ => True). intuition. cbv beta. eapply decode_correct. intro.
-    unfold encode_decode_correct.
-    intros. destruct data.
-    instantiate (1:=fun _ _ => Build_question _ _ _). simpl.
-    simpl in *. intuition. subst. reflexivity. *)
+Definition encode_question (bundle : question_t * bin_t) :=
+  encode_name (qname (fst bundle),
+    bin_encode_transform_pair (@FixInt_encode _) (FixInt_of_type (qtype (fst bundle)),
+      bin_encode_transform_pair (@FixInt_encode _) (FixInt_of_class (qclass (fst bundle)), snd bundle))).
 
-  Defined.
+Global Instance question_decoder
+  : decoder (fun _ => True) encode_question.
+Proof.
+  unfold encode_question.
 
-  Record packet :=
-    { id : Bvector 16;
-      flags : Bvector 16;
-      questions : list question;
-      answers : list question;
-      authority : list question;
-      additional : list question }.
+  eapply decode_unpack.
+  instantiate (1:=fun ls => True /\ (forall x, In x (proj1_sig ls) -> True)). intuition. cbv beta.
+  eapply name_decoder.
+  intro.
 
-End DnsPacket.
+  eapply decode_unpack with
+    (encode1:=fun bundle => bin_encode_transform_pair (FixInt_encode (size:=16))
+                              (FixInt_of_type (fst bundle), snd bundle))
+    (encode2:=fun data => bin_encode_transform_pair (FixInt_encode (size:=16))
+                            (FixInt_of_class (qclass (fst data)), snd data)).
+  instantiate (1:=fun _ => True). intuition. cbv beta.
+  eapply Nested_decoder with
+    (encodeA:=fun data => (FixInt_of_type (fst data), snd data))
+    (encodeB:=bin_encode_transform_pair (FixInt_encode (size:=16))).
+  eapply Unprod_decoder. eapply type_to_FixInt_decoder.
+  eapply bin_encode_transform_pair_Decoder. eapply FixInt_encode_correct.
+  intro.
+
+  eapply decode_unpack with
+    (encode1:=fun bundle => bin_encode_transform_pair (FixInt_encode (size:=16))
+                              (FixInt_of_class (fst bundle), snd bundle)).
+  instantiate (1:=fun _ => True). intuition. cbv beta.
+  eapply Nested_decoder with
+    (encodeA:=fun data => (FixInt_of_class (fst data), snd data))
+    (encodeB:=bin_encode_transform_pair (FixInt_encode (size:=16))).
+  eapply Unprod_decoder. eapply class_to_FixInt_decoder.
+  eapply bin_encode_transform_pair_Decoder. eapply FixInt_encode_correct.
+  intro.
+
+  eexists. instantiate (1:=fun b => (Build_question_t _ _ _, b)).
+  intro. intuition. destruct data as [rdata bin]. destruct rdata. simpl in *. subst. eauto.
+Defined.
+
+Record packet_t :=
+  { pid : { s : list bool | length s = 16 };
+    pmask : { s : list bool | length s = 16 };
+    pquestion : { s : list question_t | length s < exp2_nat 16 };
+    panswer : { s : list question_t | length s < exp2_nat 16 };
+    pauthority : { s : list question_t | length s < exp2_nat 16 };
+    padditional : { s : list question_t | length s < exp2_nat 16 } }.
+
+Definition encode_packet (bundle : packet_t * bin_t) :=
+  FixList2_encode (bin_encode_transform_pair Bool_encode) (pid (fst bundle),
+  FixList2_encode (bin_encode_transform_pair Bool_encode) (pmask (fst bundle),
+  bin_encode_transform_pair (@FixInt_encode _) (FixList_getlength (pquestion (fst bundle)),
+  bin_encode_transform_pair (@FixInt_encode _) (FixList_getlength (panswer (fst bundle)),
+  bin_encode_transform_pair (@FixInt_encode _) (FixList_getlength (pauthority (fst bundle)),
+  bin_encode_transform_pair (@FixInt_encode _) (FixList_getlength (padditional (fst bundle)),
+  FixList_encode encode_question (pquestion (fst bundle),
+  FixList_encode encode_question (panswer (fst bundle),
+  FixList_encode encode_question (pauthority (fst bundle),
+  FixList_encode encode_question (padditional (fst bundle), snd bundle)))))))))).
+
+Global Instance packet_decoder
+  : decoder (fun _ => True) encode_packet.
+Proof.
+  unfold encode_packet.
+
+  eapply decode_unpack.
+  instantiate (1:=fun ls => forall x, In x (proj1_sig ls) -> True). intuition. cbv beta.
+  eapply FixList2_decoder.
+  eapply bin_encode_transform_pair_Decoder. eapply Bool_encode_correct.
+  intro.
+
+  eapply decode_unpack.
+  instantiate (1:=fun ls => forall x, In x (proj1_sig ls) -> True). intuition. cbv beta.
+  eapply FixList2_decoder.
+  eapply bin_encode_transform_pair_Decoder. eapply Bool_encode_correct.
+  intro.
+
+  eapply decode_unpack.
+  instantiate (1:=fun _ => True). intuition. cbv beta.
+  eapply bin_encode_transform_pair_Decoder. eapply FixInt_encode_correct.
+  intro.
+
+  eapply decode_unpack.
+  instantiate (1:=fun _ => True). intuition. cbv beta.
+  eapply bin_encode_transform_pair_Decoder. eapply FixInt_encode_correct.
+  intro.
+
+  eapply decode_unpack.
+  instantiate (1:=fun _ => True). intuition. cbv beta.
+  eapply bin_encode_transform_pair_Decoder. eapply FixInt_encode_correct.
+  intro.
+
+  eapply decode_unpack.
+  instantiate (1:=fun _ => True). intuition. cbv beta.
+  eapply bin_encode_transform_pair_Decoder. eapply FixInt_encode_correct.
+  intro.
+
+  eapply decode_unpack with
+    (encode1:=FixList_encode encode_question).
+  instantiate (1:=fun data => FixList_getlength data = proj1 /\
+                              forall x, In x (proj1_sig data) -> True). intuition. cbv beta.
+  eapply FixList_decoder.
+  eapply question_decoder.
+  intro.
+  eapply decode_unpack with
+    (encode1:=FixList_encode encode_question).
+  instantiate (1:=fun data => FixList_getlength data = proj2 /\
+                              forall x, In x (proj1_sig data) -> True). intuition. cbv beta.
+  eapply FixList_decoder.
+  eapply question_decoder.
+  intro.
+  eapply decode_unpack with
+    (encode1:=FixList_encode encode_question).
+  instantiate (1:=fun data => FixList_getlength data = proj3 /\
+                              forall x, In x (proj1_sig data) -> True). intuition. cbv beta.
+  eapply FixList_decoder.
+  eapply question_decoder.
+  intro.
+  eapply decode_unpack with
+    (encode1:=FixList_encode encode_question).
+  instantiate (1:=fun data => FixList_getlength data = proj4 /\
+                              forall x, In x (proj1_sig data) -> True). intuition. cbv beta.
+  eapply FixList_decoder.
+  eapply question_decoder.
+  intro.
+
+  eexists. instantiate (1:=fun b => (Build_packet_t _ _ _ _ _ _, b)).
+  intro. intuition. destruct data as [rdata bin]. destruct rdata. simpl in *. subst. eauto.
+Defined.
+
+Extract Inductive bool => "bool" [ "true" "false" ].
+Extract Inductive sumbool => "bool" [ "true" "false" ].
+Extract Inductive list => "list" [ "[]" "(::)" ].
+Extract Inductive prod => "(*)"  [ "(,)" ].
+Extract Inductive ascii => char [
+"(* If this appears, you're using Ascii internals. Please don't *) (fun (b0,b1,b2,b3,b4,b5,b6,b7) → let f b i = if b then 1 lsl i else 0 in Char.chr (f b0 0 + f b1 1 + f b2 2 + f b3 3 + f b4 4 + f b5 5 + f b6 6 + f b7 7))"
+]
+"(* If this appears, you're using Ascii internals. Please don't *) (fun f c → let n = Char.code c in let h i = (n land (1 lsl i)) ≠ 0 in f (h 0) (h 1) (h 2) (h 3) (h 4) (h 5) (h 6) (h 7))".
+Recursive Extraction packet_decoder.
