src/BinEncoders/Libraries/Char.v
@@ -1,68 +1,28 @@
 Require Export Coq.Strings.Ascii.
-Require Import Coq.omega.Omega.
-Require Import Fiat.BinEncoders.Specs
-               Fiat.BinEncoders.Libraries.Core
+Require Import Coq.omega.Omega
+               Fiat.BinEncoders.Specs
+               Fiat.BinEncoders.Libraries.BinCore
                Fiat.BinEncoders.Libraries.FixInt.
 
-Section Char_encode_decode.
-
-  Lemma nonzero_8 : 0 < 8. omega. Qed.
-
-  Definition Char_encode_pair (p : ascii * bin) : bin.
-    refine (FixInt_encode_pair 8 (exist _ (N_of_ascii (fst p)) _, snd p)).
+Section CharBinEncoder.
+  Definition Char_encode (c : ascii) : bin_t.
+    refine (@FixInt_encode 8 (exist _ (N_of_ascii c) _)).
     unfold exp2; unfold exp2'.
-    induction (fst p).
+    induction c.
     repeat (match goal with
               | B : bool |- _ => destruct B
             end); simpl; unfold Nlt; auto.
   Defined.
 
-  Definition Char_encode (c : ascii) := Char_encode_pair (c, nil).
+  Definition Char_decode b :=
+    let (n, ext) := FixInt_decode 8 b
+    in  (ascii_of_N (proj1_sig n), ext).
 
-  Definition Char_decode_pair (b : bin) : ascii * bin :=
-    let (_n, _bin) := @Specs.decode _ _ _ _ (FixInt_decoder_pair 8) b
-    in  (ascii_of_N (proj1_sig _n), _bin).
-
-  Definition Char_decode (b : bin) : ascii := fst (Char_decode_pair b).
-
-  Theorem Char_encode_decode_correct_pair :
-    encode_decode_correct (fun _ => True) Char_encode_pair Char_decode_pair.
+  Theorem Char_encode_correct : bin_encode_correct Char_encode Char_decode.
   Proof.
-    unfold encode_decode_correct, Char_encode_pair, Char_decode_pair.
-    intros c _.
-    rewrite (@decode_correct _ _ _ (FixInt_encode_pair 8) _); simpl; eauto.
-    rewrite ascii_N_embedding; intuition.
+    unfold bin_encode_correct, Char_encode, Char_decode.
+    intros c ext.
+    rewrite FixInt_encode_correct; simpl.
+    rewrite ascii_N_embedding. reflexivity.
   Qed.
-
-  Theorem Char_encode_decode_correct :
-    encode_decode_correct (fun _ => True) Char_encode Char_decode.
-  Proof.
-    unfold encode_decode_correct, Char_encode, Char_decode.
-    intros c _.
-    rewrite Char_encode_decode_correct_pair; intuition.
-  Qed.
-
-  (* Theorem decode_shorten : decode_shorten decode.
-  Proof.
-    unfold decode_shorten, decode; intro ls.
-    pose proof (shorten_R (FixInt_encode_decode 8 nonzero_8) ls).
-    destruct (decode_R (FixInt_encode_decode 8 nonzero_8) ls); eauto.
-  Qed.
-
-  Definition Char_encode_decode :=
-    {| predicate_R := fun _ => True;
-       encode_R    := encode;
-       decode_R    := decode;
-       proof_R     := encode_correct;
-       shorten_R   := decode_shorten |}. *)
-End Char_encode_decode.
-
-Global Instance Char_decoder
-  : decoder (fun _ => True) Char_encode :=
-  { decode := Char_decode;
-    decode_correct := Char_encode_decode_correct }.
-
-Global Instance Char_decoder_pair
-  : decoder (fun _ => True) Char_encode_pair :=
-  { decode := Char_decode_pair;
-    decode_correct := Char_encode_decode_correct_pair }.
+End CharBinEncoder.
