src/BinEncoders/Libraries/Bool.v
@@ -1,0 +1,18 @@
+Require Import Fiat.BinEncoders.Specs
+               Fiat.BinEncoders.Libraries.BinCore.
+
+Section BoolBinEncoder.
+  Definition Bool_encode (b : bool) : bin_t := b :: nil.
+
+  Definition Bool_decode (b : bin_t) : bool * bin_t :=
+    match b with
+    | nil => (false, nil) (* bogus *)
+    | x :: xs => (x, xs)
+    end.
+
+  Theorem Bool_encode_correct : bin_encode_correct Bool_encode Bool_decode.
+  Proof.
+    unfold bin_encode_correct, Bool_encode, Bool_decode.
+    eauto.
+  Qed.
+End BoolBinEncoder.
